`LGS.v`: Thompson's Construction.

theories/System/LGS.v
@@ -459,9 +459,1508 @@ Proof.
     + subst bad_rule. simpl. unfold compileRule at 1. rewrite NULLABLE. ss!.
     + simpl. destruct (compileRule rule) as [[idx] | compiled_rule] eqn: COMPILE_RULE; simpl; eauto.
       pose proof (IH (@ex_intro _ _ bad_rule (conj IN NULLABLE))) as (idx & FAILURE); simpl.
-      rewrite FAILURE; exists idx; reflexivity.
+      now rewrite FAILURE; exists idx.
 Qed.
 
 End Rule.
+
+Module TaggedENFA.
+
+#[projections(primitive)]
+Record t : Type :=
+  mk
+  { state : Set
+  ; state_hasEqDec : hasEqDec@{Set} state
+  ; states : list state
+  ; start_state : state
+  ; accept_states : list (state * Token.t)
+  ; eps_step (q : state) : list state
+  ; char_step (q : state) (c : ascii) : list state
+  } as M.
+
+#[global] Existing Instance state_hasEqDec.
+
+Variant okay (M : TaggedENFA.t) : Prop :=
+  | okay_intro
+    (start_okay : M.(TaggedENFA.start_state) ∈ M.(TaggedENFA.states))
+    (accept_states_okay : forall q, forall tag, (q, tag) ∈ M.(TaggedENFA.accept_states) -> q ∈ M.(TaggedENFA.states))
+    (eps_step_okay : forall q, forall q', q ∈ M.(TaggedENFA.states) -> q' ∈ M.(TaggedENFA.eps_step) q -> q' ∈ M.(TaggedENFA.states))
+    (char_step_okay : forall q, forall q', forall c, q ∈ M.(TaggedENFA.states) -> q' ∈ M.(TaggedENFA.char_step) q c -> q' ∈ M.(TaggedENFA.states)).
+
+Section DELTA_STAR.
+
+Context {Q : Type}.
+
+Variable eps_step : Q -> list Q.
+
+Inductive eclosure (q : Q) : ensemble Q :=
+  | eclosure_refl
+    : q \in eclosure q
+  | eclosure_step q1 q2
+    (STEP : q1 ∈ eps_step q)
+    (REST : q2 \in eclosure q1)
+    : q2 \in eclosure q.
+
+#[local] Hint Constructors eclosure : core.
+
+Lemma eclosure_trans (q1 : Q) (q2 : Q) (q3 : Q)
+  (H1_eclosure : q2 \in eclosure q1)
+  (H2_eclosure : q3 \in eclosure q2)
+  : q3 \in eclosure q1.
+Proof.
+  induction H1_eclosure as [q | q q1' q2' STEP REST IH]; simpl; eauto with *.
+Qed.
+
+Variable char_step : Q -> ascii -> list Q.
+
+Inductive delta_star (q : Q) : Input.t -> ensemble Q :=
+  | delta_star_nil
+    : q \in delta_star q []
+  | delta_star_eps q1 q2 s
+    (STEP : q1 ∈ eps_step q)
+    (REST : q2 \in delta_star q1 s)
+    : q2 \in delta_star q s
+  | delta_star_char q1 q2 c s
+    (STEP : q1 ∈ char_step q c)
+    (REST : q2 \in delta_star q1 s)
+    : q2 \in delta_star q (c :: s).
+
+#[local] Hint Constructors delta_star : core.
+
+Lemma delta_star_app (q1 : Q) (q2 : Q) (q3 : Q) (s1 : Input.t) (s2 : Input.t)
+  (H1_delta_star : q2 \in delta_star q1 s1)
+  (H2_delta_star : q3 \in delta_star q2 s2)
+  : q3 \in delta_star q1 (s1 ++ s2).
+Proof.
+  induction H1_delta_star as [q | q q1' q2' s STEP REST IH | q q1' q2' c s STEP REST IH]; simpl; eauto with *.
+Qed.
+
+Lemma delta_star_iff_eclosure (q : Q) (q' : Q)
+  : q' \in delta_star q [] <-> q' \in eclosure q.
+Proof.
+  split; [intros H_delta_star | intros H_eclosure].
+  - remember (@nil ascii) as s eqn: EQ; induction H_delta_star as [q | q q1' q2' s STEP REST IH | q q1' q2' c s STEP REST IH]; inv EQ; simpl; eauto with *.
+  - induction H_eclosure as [q | q q1' q2' STEP REST IH]; simpl; eauto with *.
+Qed.
+
+Lemma delta_star_elim (q1 : Q) (q3 : Q) (s : Input.t)
+  (H_delta_star : q3 \in delta_star q1 s)
+  : ⟪ DELTA_STAR_NIL : s = [] /\ q3 = q1 ⟫ \/ ⟪ DELTA_STAR_EPS : exists q2, q2 ∈ eps_step q1 /\ q3 \in delta_star q2 s ⟫ \/ ⟪ DELTA_STAR_CHAR : exists c, exists s', exists q2, s = c :: s' /\ q2 ∈ char_step q1 c /\ q3 \in delta_star q2 s' ⟫.
+Proof.
+  unnw; destruct H_delta_star as [ | q1' q2' s' STEP REST | q1' q2' c s' STEP REST]; [left | right; left | right; right]; done!.
+Qed.
+
+Lemma delta_star_stuck (q1 : Q) (q2 : Q) (s : Input.t)
+  (NO_EPS : forall q, ~ (q ∈ eps_step q1))
+  (NO_CHAR : forall c, forall q, ~ (q ∈ char_step q1 c))
+  (H_delta_star : q2 \in delta_star q1 s)
+  : s = [] /\ q2 = q1.
+Proof.
+  inv H_delta_star; ss!.
+Qed.
+
+End DELTA_STAR.
+
+Section BASICS.
+
+Variable M : TaggedENFA.t.
+
+#[local] Abbreviation Q := M.(TaggedENFA.state).
+#[local] Abbreviation M_delta_star := (delta_star M.(TaggedENFA.eps_step) M.(TaggedENFA.char_step)).
+#[local] Abbreviation M_eclosure := (eclosure M.(TaggedENFA.eps_step)).
+
+Lemma eclosure_okay (q1 : Q) (q2 : Q)
+  (OKAY : TaggedENFA.okay M)
+  (IN : q1 ∈ M.(TaggedENFA.states))
+  (H_eclosure : q2 \in M_eclosure q1)
+  : q2 ∈ M.(TaggedENFA.states).
+Proof.
+  destruct OKAY as [_ _ ? _]; induction H_eclosure as [q | q q1' q2' STEP REST IH]; simpl; eauto with *.
+Qed.
+
+Lemma delta_star_okay (q1 : Q) (q2 : Q) (s : Input.t)
+  (OKAY : TaggedENFA.okay M)
+  (IN : q1 ∈ M.(TaggedENFA.states))
+  (H_delta_star : q2 \in M_delta_star q1 s)
+  : q2 ∈ M.(TaggedENFA.states).
+Proof.
+  destruct OKAY as [_ _ ? ?]; induction H_delta_star as [q | q q1' q2' s STEP REST IH | q q1' q2' c s STEP REST IH]; simpl; eauto with *.
+Qed.
+
+Definition accepts (s : Input.t) (tag : Token.t) : Prop :=
+  exists qf, qf \in M_delta_star M.(TaggedENFA.start_state) s /\ (qf, tag) ∈ M.(TaggedENFA.accept_states).
+
+Definition accepted_tags (s : Input.t) : ensemble Token.t :=
+  fun tag => accepts s tag.
+
+End BASICS.
+
+Section Thompson's_construction.
+
+#[projections(primitive)]
+Record char_edge : Set :=
+  mkCharEdge
+  { char_edge_src : nat
+  ; char_edge_label : ascii
+  ; char_edge_dst : nat
+  } as char_edge.
+
+#[projections(primitive)]
+Record fragment : Set :=
+  mkFragment
+  { frag_start : nat
+  ; frag_accept : nat
+  ; frag_eps_edges : list (nat * nat)
+  ; frag_char_edges : list char_edge
+  } as frag.
+
+Fixpoint regex2fragment (e : regex ascii) (qi : nat) {struct e} : nat * fragment :=
+  match e with
+  | Re.Null =>
+    let qf := qi + 1 in
+    (qf, mkFragment qi qf [] [])
+  | Re.Empty =>
+    let qf := qi + 1 in
+    (qf, mkFragment qi qf [(qi, qf)] [])
+  | Re.Char c =>
+    let qf := qi + 1 in
+    (qf, mkFragment qi qf [] [mkCharEdge qi c qf])
+  | Re.Union e1 e2 =>
+    let qi1 := qi + 1 in
+    let '(qf1, frag1) := regex2fragment e1 qi1 in
+    let qi2 := qf1 + 1 in
+    let '(qf2, frag2) := regex2fragment e2 qi2 in
+    let qf := qf2 + 1 in
+    (qf, mkFragment qi qf ((qi, qi1) :: (qi, qi2) :: (qf1, qf) :: (qf2, qf) :: frag1.(frag_eps_edges) ++ frag2.(frag_eps_edges)) (frag1.(frag_char_edges) ++ frag2.(frag_char_edges)))
+  | Re.Append e1 e2 =>
+    let qi1 := qi + 1 in
+    let '(qf1, frag1) := regex2fragment e1 qi1 in
+    let qi2 := qf1 + 1 in
+    let '(qf2, frag2) := regex2fragment e2 qi2 in
+    let qf := qf2 + 1 in
+    (qf, mkFragment qi qf ((qi, qi1) :: (qf1, qi2) :: (qf2, qf) :: frag1.(frag_eps_edges) ++ frag2.(frag_eps_edges)) (frag1.(frag_char_edges) ++ frag2.(frag_char_edges)))
+  | Re.Star e1 =>
+    let qi1 := qi + 1 in
+    let '(qf1, frag1) := regex2fragment e1 qi1 in
+    let qf := qf1 + 1 in
+    (qf, mkFragment qi qf ((qi, qi1) :: (qf1, qi1) :: (qi1, qf) :: frag1.(frag_eps_edges)) frag1.(frag_char_edges))
+  end.
+
+Fixpoint rules2fragments (qi : nat) (rules : list Rule.t) {struct rules} : nat * list (Rule.t * fragment) :=
+  match rules with
+  | [] => (qi, [])
+  | rule :: rules' =>
+    let '(qf, frag) := regex2fragment rule.(Rule.regex) qi in
+    let '(qmax, frags) := rules2fragments (qf + 1) rules' in
+    (qmax, (rule, frag) :: frags)
+  end.
+
+Fixpoint eps_step_from_edges (q : nat) (edges : list (nat * nat)) {struct edges} : list nat :=
+  match edges with
+  | [] => []
+  | (src, dst) :: edges' =>
+    if eq_dec q src then
+      dst :: eps_step_from_edges q edges'
+    else
+      eps_step_from_edges q edges'
+  end.
+
+Fixpoint char_step_from_edges (q : nat) (c : ascii) (edges : list char_edge) {struct edges} : list nat :=
+  match edges with
+  | [] => []
+  | edge :: edges' =>
+    if eq_dec q edge.(char_edge_src) then
+      if eq_dec c edge.(char_edge_label) then
+        edge.(char_edge_dst) :: char_step_from_edges q c edges'
+      else
+        char_step_from_edges q c edges'
+    else
+      char_step_from_edges q c edges'
+  end.
+
+Fixpoint fragment_eps_edges (frags : list (Rule.t * fragment)) {struct frags} : list (nat * nat) :=
+  match frags with
+  | [] => []
+  | (_, frag) :: frags' => (0, frag.(frag_start)) :: frag.(frag_eps_edges) ++ fragment_eps_edges frags'
+  end.
+
+Fixpoint fragment_char_edges (frags : list (Rule.t * fragment)) {struct frags} : list char_edge :=
+  match frags with
+  | [] => []
+  | (_, frag) :: frags' => frag.(frag_char_edges) ++ fragment_char_edges frags'
+  end.
+
+Definition fragment_accept_states (frags : list (Rule.t * fragment)) : list (nat * Token.t) :=
+  map (fun '(rule, frag) => (frag.(frag_accept), rule.(Rule.token))) frags.
+
+Definition fragments2TaggedENFA (qmax : nat) (frags : list (Rule.t * fragment)) : TaggedENFA.t :=
+  let eps_edges := fragment_eps_edges frags in
+  let char_edges := fragment_char_edges frags in
+  {|
+    state := nat;
+    state_hasEqDec := nat_hasEqDec;
+    states := seq 0 qmax;
+    start_state := 0;
+    accept_states := fragment_accept_states frags;
+    eps_step := fun q => eps_step_from_edges q eps_edges;
+    char_step := fun q => fun c => char_step_from_edges q c char_edges;
+  |}.
+
+Definition mkUnitedTaggedENFA (rules : list Rule.t) : TaggedENFA.t :=
+  let '(qmax, frags) := rules2fragments 1 rules in
+  fragments2TaggedENFA qmax frags.
+
+Lemma eps_step_from_edges_complete (q : nat) (q' : nat) (edges : list (nat * nat))
+  (IN : (q, q') ∈ edges)
+  : q' ∈ eps_step_from_edges q edges.
+Proof.
+  induction edges as [ | [src dst] edges IH]; simpl in IN |- *; des; des_ifs; ss!.
+Qed.
+
+Lemma eps_step_from_edges_sound (q : nat) (q' : nat) (edges : list (nat * nat))
+  (IN : q' ∈ eps_step_from_edges q edges)
+  : (q, q') ∈ edges.
+Proof.
+  induction edges as [ | [src dst] edges IH]; simpl in IN |- *; des; des_ifs; ss!.
+Qed.
+
+Lemma char_step_from_edges_complete (edge : char_edge) (edges : list char_edge)
+  (IN : edge ∈ edges)
+  : edge.(char_edge_dst) ∈ char_step_from_edges edge.(char_edge_src) edge.(char_edge_label) edges.
+Proof.
+  induction edges as [ | edge' edges IH]; simpl in IN |- *; des; des_ifs; ss!.
+Qed.
+
+Lemma char_step_from_edges_sound (q : nat) (q' : nat) (c : ascii) (edges : list char_edge)
+  (IN : q' ∈ char_step_from_edges q c edges)
+  : exists edge, edge ∈ edges /\ edge.(char_edge_src) = q /\ edge.(char_edge_label) = c /\ edge.(char_edge_dst) = q'.
+Proof.
+  induction edges as [ | edge edges IH]; simpl in IN |- *; try tauto.
+  destruct (eq_dec q edge.(char_edge_src)) as [SRC_EQ | SRC_NE].
+  - destruct (eq_dec c edge.(char_edge_label)) as [LABEL_EQ | LABEL_NE]; simpl in IN.
+    + destruct IN as [DST_EQ | IN].
+      * exists edge; ss!.
+      * pose proof (IH IN) as (edge' & IN_EDGE & SRC' & LABEL' & DST'). exists edge'; ss!.
+    + pose proof (IH IN) as (edge' & IN_EDGE & SRC' & LABEL' & DST'). exists edge'; ss!.
+  - pose proof (IH IN) as (edge' & IN_EDGE & SRC' & LABEL' & DST'). exists edge'; ss!.
+Qed.
+
+Lemma fragment_eps_edges_start_complete (frags : list (Rule.t * fragment)) (rule : Rule.t) (frag : fragment)
+  (IN : (rule, frag) ∈ frags)
+  : (0, frag.(frag_start)) ∈ fragment_eps_edges frags.
+Proof.
+  induction frags as [ | [rule' frag'] frags IH]; simpl in IN |- *; ss!.
+Qed.
+
+Lemma fragment_eps_edges_complete (frags : list (Rule.t * fragment)) (rule : Rule.t) (frag : fragment) (q : nat) (q' : nat)
+  (IN_FRAG : (rule, frag) ∈ frags)
+  (IN_EDGE : (q, q') ∈ frag.(frag_eps_edges))
+  : (q, q') ∈ fragment_eps_edges frags.
+Proof.
+  induction frags as [ | [rule' frag'] frags IH]; simpl in IN_FRAG |- *; des; ss!.
+Qed.
+
+Lemma fragment_char_edges_complete (frags : list (Rule.t * fragment)) (rule : Rule.t) (frag : fragment) (edge : char_edge)
+  (IN_FRAG : (rule, frag) ∈ frags)
+  (IN_EDGE : edge ∈ frag.(frag_char_edges))
+  : edge ∈ fragment_char_edges frags.
+Proof.
+  induction frags as [ | [rule' frag'] frags IH]; simpl in IN_FRAG |- *; des; ss!.
+Qed.
+
+Lemma fragment_accept_states_complete (frags : list (Rule.t * fragment)) (rule : Rule.t) (frag : fragment)
+  (IN_FRAG : (rule, frag) ∈ frags)
+  : (frag.(frag_accept), rule.(Rule.token)) ∈ fragment_accept_states frags.
+Proof.
+  unfold fragment_accept_states. ss!.
+Qed.
+
+Lemma fragment_accept_states_sound (frags : list (Rule.t * fragment)) q tag
+  (IN : (q, tag) ∈ fragment_accept_states frags)
+  : exists rule, exists frag, (rule, frag) ∈ frags /\ q = frag.(frag_accept) /\ tag = rule.(Rule.token).
+Proof.
+  unfold fragment_accept_states in IN. rewrite L.in_map_iff in IN.
+  destruct IN as ([rule frag] & EQ & IN_FRAG). inv EQ. now exists rule, frag.
+Qed.
+
+Variant TaggedENFA_COMPILED (M : TaggedENFA.t) (rules : list Rule.t) (qmax : nat) (frags : list (Rule.t * fragment)) : Prop :=
+  | TaggedENFA_COMPILED_intro 
+    (COMPILED_RULES : Rule.compileds = inr rules)
+    (COMPILED_ENFA : M = mkUnitedTaggedENFA rules)
+    (COMPILED_FRAGS : rules2fragments 1 rules = (qmax, frags)).
+
+Variant TaggedENFA_FRAGMENTS (frags : list (Rule.t * fragment)) (rule : Rule.t) (frag : fragment) : Prop :=
+  | TaggedENFA_FRAGMENTS_intro
+    (start_in : frag.(frag_start) ∈ eps_step_from_edges 0 (fragment_eps_edges frags))
+    (accept_in : (frag.(frag_accept), rule.(Rule.token)) ∈ fragment_accept_states frags)
+    (eps_in : forall q, forall q', (q, q') ∈ frag.(frag_eps_edges) -> q' ∈ eps_step_from_edges q (fragment_eps_edges frags))
+    (char_in : forall edge, edge ∈ frag.(frag_char_edges) -> edge.(char_edge_dst) ∈ char_step_from_edges edge.(char_edge_src) edge.(char_edge_label) (fragment_char_edges frags)).
+
+Theorem mkUnitedTaggedENFA_spec (M : TaggedENFA.t)
+  (COMPILE : fmap mkUnitedTaggedENFA Rule.compileds = inr M)
+  : exists rules, exists qmax, exists frags, TaggedENFA_COMPILED M rules qmax frags /\ (forall rule, forall frag, (rule, frag) ∈ frags -> TaggedENFA_FRAGMENTS frags rule frag).
+Proof.
+  unfold fmap, mkFunctorFromMonad in COMPILE. simpl in COMPILE.
+  destruct Rule.compileds as [err | rules] eqn: COMPILED; inv COMPILE.
+  destruct (rules2fragments 1 rules) as [qmax frags] eqn: FRAGS.
+  exists rules, qmax, frags. split.
+  - split; eauto.
+  - ii; split; i.
+    + eapply eps_step_from_edges_complete. eapply fragment_eps_edges_start_complete; eauto.
+    + eapply fragment_accept_states_complete; eauto.
+    + eapply eps_step_from_edges_complete. eapply fragment_eps_edges_complete; eauto.
+    + eapply char_step_from_edges_complete. eapply fragment_char_edges_complete; eauto.
+Qed.
+
+Definition fragments_delta_star (frags : list (Rule.t * fragment)) : nat -> Input.t -> ensemble nat :=
+  delta_star (fun q => eps_step_from_edges q (fragment_eps_edges frags)) (fun q => fun c => char_step_from_edges q c (fragment_char_edges frags)).
+
+Definition fragment_delta_star (frag : fragment) : nat -> Input.t -> ensemble nat :=
+  delta_star (fun q => eps_step_from_edges q frag.(frag_eps_edges)) (fun q => fun c => char_step_from_edges q c frag.(frag_char_edges)).
+
+Lemma mkUnitedTaggedENFA_unfold_fragments rules qmax frags
+  (FRAGS : rules2fragments 1 rules = (qmax, frags))
+  : mkUnitedTaggedENFA rules = fragments2TaggedENFA qmax frags.
+Proof.
+  unfold mkUnitedTaggedENFA, fragments2TaggedENFA. rewrite FRAGS. reflexivity.
+Qed.
+
+Lemma TaggedENFA_COMPILED_as_fragments M rules qmax frags
+  (COMPILED : TaggedENFA_COMPILED M rules qmax frags)
+  : M = fragments2TaggedENFA qmax frags.
+Proof.
+  inv COMPILED. eapply mkUnitedTaggedENFA_unfold_fragments. exact COMPILED_FRAGS.
+Qed.
+
+Lemma TaggedENFA_FRAGMENTS_delta_star_step frags rule frag
+  (FRAGMENTS : TaggedENFA_FRAGMENTS frags rule frag)
+  : ⟪ EPS : forall q, forall q', (q, q') ∈ frag.(frag_eps_edges) -> q' \in fragments_delta_star frags q [] ⟫ /\ ⟪ CHAR : forall edge, edge ∈ frag.(frag_char_edges) -> edge.(char_edge_dst) \in fragments_delta_star frags edge.(char_edge_src) [edge.(char_edge_label)] ⟫.
+Proof.
+  destruct FRAGMENTS as [_ _ EPS CHAR]. split.
+  - intros q q' IN_EDGE. eapply delta_star_eps with (q1 := q').
+    + exact (EPS q q' IN_EDGE).
+    + econs.
+  - intros edge IN_EDGE. eapply delta_star_char with (q1 := edge.(char_edge_dst)).
+    + exact (CHAR edge IN_EDGE).
+    + econs.
+Qed.
+
+Lemma regex2fragment_empty_delta_star frags rule qi qf frag
+  (REGEX2FRAGMENT : regex2fragment Re.Empty qi = (qf, frag))
+  (FRAGMENTS : TaggedENFA_FRAGMENTS frags rule frag)
+  : frag.(frag_accept) \in fragments_delta_star frags frag.(frag_start) [].
+Proof.
+  pose proof (TaggedENFA_FRAGMENTS_delta_star_step frags rule frag FRAGMENTS) as [EPS _].
+  simpl in REGEX2FRAGMENT. inv REGEX2FRAGMENT. eapply EPS. simpl. left. reflexivity.
+Qed.
+
+Lemma regex2fragment_start_accept e qi qf frag
+  (REGEX2FRAGMENT : regex2fragment e qi = (qf, frag))
+  : frag.(frag_start) = qi /\ frag.(frag_accept) = qf.
+Proof.
+  revert qi qf frag REGEX2FRAGMENT.
+  induction e as [ | | c | e1 IH1 e2 IH2 | e1 IH1 e2 IH2 | e IH]; intros qi qf frag REGEX2FRAGMENT; simpl in REGEX2FRAGMENT.
+  - inv REGEX2FRAGMENT. eauto.
+  - inv REGEX2FRAGMENT. eauto.
+  - inv REGEX2FRAGMENT. eauto.
+  - destruct (regex2fragment e1 (qi + 1)) as [qf1 frag1].
+    destruct (regex2fragment e2 (qf1 + 1)) as [qf2 frag2].
+    inv REGEX2FRAGMENT. eauto.
+  - destruct (regex2fragment e1 (qi + 1)) as [qf1 frag1].
+    destruct (regex2fragment e2 (qf1 + 1)) as [qf2 frag2].
+    inv REGEX2FRAGMENT. eauto.
+  - destruct (regex2fragment e (qi + 1)) as [qf1 frag1].
+    inv REGEX2FRAGMENT. eauto.
+Qed.
+
+Lemma regex2fragment_same_fragment e qi1 qf1 qi2 qf2 frag
+  (REGEX1 : regex2fragment e qi1 = (qf1, frag))
+  (REGEX2 : regex2fragment e qi2 = (qf2, frag))
+  : qi1 = qi2 /\ qf1 = qf2.
+Proof.
+  pose proof (regex2fragment_start_accept _ _ _ _ REGEX1) as [START1 ACCEPT1].
+  pose proof (regex2fragment_start_accept _ _ _ _ REGEX2) as [START2 ACCEPT2].
+  split; congruence.
+Qed.
+
+Definition eps_edge_in_range (lo : nat) (hi : nat) (edge : nat * nat) : Prop :=
+  lo <= fst edge <= hi /\ lo <= snd edge <= hi.
+
+Definition char_edge_in_range (lo : nat) (hi : nat) (edge : char_edge) : Prop :=
+  lo <= edge.(char_edge_src) <= hi /\ lo <= edge.(char_edge_dst) <= hi.
+
+Variant FRAGMENT_BOUNDS (lo : nat) (hi : nat) (frag : fragment) : Prop :=
+  | FRAGMENT_BOUNDS_intro
+    (BOUNDS_START : frag.(frag_start) = lo)
+    (BOUNDS_ACCEPT : frag.(frag_accept) = hi)
+    (BOUNDS_LT : lo < hi)
+    (BOUNDS_EPS : forall edge, edge ∈ frag.(frag_eps_edges) -> eps_edge_in_range lo hi edge)
+    (BOUNDS_CHAR : forall edge, edge ∈ frag.(frag_char_edges) -> char_edge_in_range lo hi edge).
+
+Lemma regex2fragment_bounds e qi qf frag
+  (REGEX2FRAGMENT : regex2fragment e qi = (qf, frag))
+  : FRAGMENT_BOUNDS qi qf frag.
+Proof.
+  revert qi qf frag REGEX2FRAGMENT.
+  induction e as [ | | c | e1 IH1 e2 IH2 | e1 IH1 e2 IH2 | e IH]; intros qi qf frag REGEX2FRAGMENT; simpl in REGEX2FRAGMENT.
+  - inv REGEX2FRAGMENT. econs; simpl; try lia; tauto.
+  - inv REGEX2FRAGMENT. econs; simpl; try lia.
+    intros [q q'] [EQ | IN]; s!; des; subst.
+    + unfold eps_edge_in_range. simpl. lia.
+    + contradiction.
+  - inv REGEX2FRAGMENT. econs; simpl; try lia.
+    intros edge [EQ | IN]; [subst edge; unfold char_edge_in_range; simpl; lia | contradiction].
+  - destruct (regex2fragment e1 (qi + 1)) as [qf1 frag1] eqn: REGEX1.
+    destruct (regex2fragment e2 (qf1 + 1)) as [qf2 frag2] eqn: REGEX2.
+    pose proof (IH1 _ _ _ REGEX1) as [START1 ACCEPT1 LT1 EPS1 CHAR1].
+    pose proof (IH2 _ _ _ REGEX2) as [START2 ACCEPT2 LT2 EPS2 CHAR2].
+    inv REGEX2FRAGMENT. econs; simpl; try lia.
+    + intros [q q'] IN_EDGE. simpl in IN_EDGE.
+      destruct IN_EDGE as [EQ | [EQ | [EQ | [EQ | IN_EDGE]]]]; s!; des; subst.
+      * unfold eps_edge_in_range. simpl. lia.
+      * unfold eps_edge_in_range. simpl. lia.
+      * unfold eps_edge_in_range. simpl. lia.
+      * unfold eps_edge_in_range. simpl. lia.
+      * pose proof (EPS1 _ IN_EDGE). unfold eps_edge_in_range in *. simpl in *. lia.
+      * pose proof (EPS2 _ IN_EDGE). unfold eps_edge_in_range in *. simpl in *. lia.
+    + intros edge IN_EDGE. simpl in IN_EDGE. rewrite in_app_iff in IN_EDGE.
+      destruct IN_EDGE as [IN_EDGE | IN_EDGE].
+      * pose proof (CHAR1 _ IN_EDGE). unfold char_edge_in_range in *. lia.
+      * pose proof (CHAR2 _ IN_EDGE). unfold char_edge_in_range in *. lia.
+  - destruct (regex2fragment e1 (qi + 1)) as [qf1 frag1] eqn: REGEX1.
+    destruct (regex2fragment e2 (qf1 + 1)) as [qf2 frag2] eqn: REGEX2.
+    pose proof (IH1 _ _ _ REGEX1) as [START1 ACCEPT1 LT1 EPS1 CHAR1].
+    pose proof (IH2 _ _ _ REGEX2) as [START2 ACCEPT2 LT2 EPS2 CHAR2].
+    inv REGEX2FRAGMENT. econs; simpl; try lia.
+    + intros [q q'] IN_EDGE. simpl in IN_EDGE.
+      destruct IN_EDGE as [EQ | [EQ | [EQ | IN_EDGE]]]; s!; des; subst.
+      * unfold eps_edge_in_range. simpl. lia.
+      * unfold eps_edge_in_range. simpl. lia.
+      * unfold eps_edge_in_range. simpl. lia.
+      * pose proof (EPS1 _ IN_EDGE). unfold eps_edge_in_range in *. simpl in *. lia.
+      * pose proof (EPS2 _ IN_EDGE). unfold eps_edge_in_range in *. simpl in *. lia.
+    + intros edge IN_EDGE. simpl in IN_EDGE. s!; des.
+      * pose proof (CHAR1 _ IN_EDGE). unfold char_edge_in_range in *. lia.
+      * pose proof (CHAR2 _ IN_EDGE). unfold char_edge_in_range in *. lia.
+  - destruct (regex2fragment e (qi + 1)) as [qf1 frag1] eqn: REGEX1.
+    pose proof (IH _ _ _ REGEX1) as [START1 ACCEPT1 LT1 EPS1 CHAR1].
+    inv REGEX2FRAGMENT. econs; simpl; try lia.
+    + intros [q q'] IN_EDGE. simpl in IN_EDGE.
+      destruct IN_EDGE as [EQ | [EQ | [EQ | IN_EDGE]]]; s!; des; subst.
+      * unfold eps_edge_in_range. simpl. lia.
+      * unfold eps_edge_in_range. simpl. lia.
+      * unfold eps_edge_in_range. simpl. lia.
+      * pose proof (EPS1 _ IN_EDGE). unfold eps_edge_in_range in *. simpl in *. lia.
+    + intros edge IN_EDGE.
+      pose proof (CHAR1 _ IN_EDGE). unfold char_edge_in_range in *. lia.
+Qed.
+
+Lemma regex2fragment_edge_src_lt e qi qf frag
+  (REGEX2FRAGMENT : regex2fragment e qi = (qf, frag))
+  : (forall q, forall q', (q, q') ∈ frag.(frag_eps_edges) -> q < qf) /\ (forall edge, edge ∈ frag.(frag_char_edges) -> edge.(char_edge_src) < qf).
+Proof.
+  revert qi qf frag REGEX2FRAGMENT.
+  induction e as [ | | c | e1 IH1 e2 IH2 | e1 IH1 e2 IH2 | e IH]; ii; simpl in REGEX2FRAGMENT.
+  - inv REGEX2FRAGMENT. split; ii; contradiction.
+  - inv REGEX2FRAGMENT. split; ii; simpl in *.
+    + destruct H as [EQ | []]. inv EQ. lia.
+    + contradiction.
+  - inv REGEX2FRAGMENT. split; ii; simpl in *.
+    + contradiction.
+    + destruct H as [EQ | []]. subst edge. simpl. lia.
+  - destruct (regex2fragment e1 (qi + 1)) as [qf1 frag1] eqn: REGEX1.
+    destruct (regex2fragment e2 (qf1 + 1)) as [qf2 frag2] eqn: REGEX2.
+    pose proof (IH1 _ _ _ REGEX1) as [EPS1 CHAR1].
+    pose proof (IH2 _ _ _ REGEX2) as [EPS2 CHAR2].
+    pose proof (regex2fragment_bounds _ _ _ _ REGEX1) as [_ _ LT1 _ _].
+    pose proof (regex2fragment_bounds _ _ _ _ REGEX2) as [_ _ LT2 _ _].
+    inv REGEX2FRAGMENT. split; ii; simpl in *.
+    + des; try (inv H; lia). rewrite in_app_iff in H. des; eauto; [pose proof (EPS1 _ _ H) | pose proof (EPS2 _ _ H)]; lia.
+    + rewrite in_app_iff in H. des; eauto; [pose proof (CHAR1 _ H) | pose proof (CHAR2 _ H)]; lia.
+  - destruct (regex2fragment e1 (qi + 1)) as [qf1 frag1] eqn: REGEX1.
+    destruct (regex2fragment e2 (qf1 + 1)) as [qf2 frag2] eqn: REGEX2.
+    pose proof (IH1 _ _ _ REGEX1) as [EPS1 CHAR1].
+    pose proof (IH2 _ _ _ REGEX2) as [EPS2 CHAR2].
+    pose proof (regex2fragment_bounds _ _ _ _ REGEX1) as [_ _ LT1 _ _].
+    pose proof (regex2fragment_bounds _ _ _ _ REGEX2) as [_ _ LT2 _ _].
+    inv REGEX2FRAGMENT. split; ii; simpl in *.
+    + des; try (inv H; lia). rewrite in_app_iff in H. des; eauto; [pose proof (EPS1 _ _ H) | pose proof (EPS2 _ _ H)]; lia.
+    + rewrite in_app_iff in H. des; eauto; [pose proof (CHAR1 _ H) | pose proof (CHAR2 _ H)]; lia.
+  - destruct (regex2fragment e (qi + 1)) as [qf1 frag1] eqn: REGEX.
+    pose proof (IH _ _ _ REGEX) as [EPS1 CHAR1].
+    pose proof (regex2fragment_bounds _ _ _ _ REGEX) as [_ _ LT1 _ _].
+    inv REGEX2FRAGMENT. split; ii; simpl in *.
+    + des; try (inv H; lia). pose proof (EPS1 _ _ H). lia.
+    + pose proof (CHAR1 _ H). lia.
+Qed.
+
+Lemma regex2fragment_edge_dst_gt_start e qi qf frag
+  (REGEX2FRAGMENT : regex2fragment e qi = (qf, frag))
+  : (forall q, forall q', (q, q') ∈ frag.(frag_eps_edges) -> qi < q') /\ (forall edge, edge ∈ frag.(frag_char_edges) -> qi < edge.(char_edge_dst)).
+Proof.
+  revert qi qf frag REGEX2FRAGMENT.
+  induction e as [ | | c | e1 IH1 e2 IH2 | e1 IH1 e2 IH2 | e IH]; ii; simpl in REGEX2FRAGMENT.
+  - inv REGEX2FRAGMENT. split; ii; contradiction.
+  - inv REGEX2FRAGMENT. split; ii; simpl in *.
+    + destruct H as [EQ | []]. inv EQ. lia.
+    + contradiction.
+  - inv REGEX2FRAGMENT. split; ii; simpl in *.
+    + contradiction.
+    + destruct H as [EQ | []]. subst edge. simpl. lia.
+  - destruct (regex2fragment e1 (qi + 1)) as [qf1 frag1] eqn: REGEX1.
+    destruct (regex2fragment e2 (qf1 + 1)) as [qf2 frag2] eqn: REGEX2.
+    pose proof (IH1 _ _ _ REGEX1) as [EPS1 CHAR1].
+    pose proof (IH2 _ _ _ REGEX2) as [EPS2 CHAR2].
+    pose proof (regex2fragment_bounds _ _ _ _ REGEX1) as [_ _ LT1 _ _].
+    pose proof (regex2fragment_bounds _ _ _ _ REGEX2) as [_ _ LT2 _ _].
+    inv REGEX2FRAGMENT. split; ii; simpl in *.
+    + des; try (inv H; lia). rewrite in_app_iff in H. des; [pose proof (EPS1 _ _ H) | pose proof (EPS2 _ _ H)]; lia.
+    + rewrite in_app_iff in H. des; [pose proof (CHAR1 _ H) | pose proof (CHAR2 _ H)]; lia.
+  - destruct (regex2fragment e1 (qi + 1)) as [qf1 frag1] eqn: REGEX1.
+    destruct (regex2fragment e2 (qf1 + 1)) as [qf2 frag2] eqn: REGEX2.
+    pose proof (IH1 _ _ _ REGEX1) as [EPS1 CHAR1].
+    pose proof (IH2 _ _ _ REGEX2) as [EPS2 CHAR2].
+    pose proof (regex2fragment_bounds _ _ _ _ REGEX1) as [_ _ LT1 _ _].
+    pose proof (regex2fragment_bounds _ _ _ _ REGEX2) as [_ _ LT2 _ _].
+    inv REGEX2FRAGMENT. split; ii; simpl in *.
+    + des; try (inv H; lia). rewrite in_app_iff in H. des; [pose proof (EPS1 _ _ H) | pose proof (EPS2 _ _ H)]; lia.
+    + rewrite in_app_iff in H. des; [pose proof (CHAR1 _ H) | pose proof (CHAR2 _ H)]; lia.
+  - destruct (regex2fragment e (qi + 1)) as [qf1 frag1] eqn: REGEX.
+    pose proof (IH _ _ _ REGEX) as [EPS1 CHAR1].
+    pose proof (regex2fragment_bounds _ _ _ _ REGEX) as [_ _ LT1 _ _].
+    inv REGEX2FRAGMENT. split; ii; simpl in *.
+    + des; try (inv H; lia). pose proof (EPS1 _ _ H). lia.
+    + pose proof (CHAR1 _ H). lia.
+Qed.
+
+Lemma regex2fragment_complete_aux (e : regex ascii) (s : Input.t) (frags : list (Rule.t * fragment)) (rule : Rule.t) (qi : nat) (qf : nat) (frag : fragment) (topfrag : fragment)
+  (IN_REGEX : s \in eval_regex e)
+  (REGEX2FRAGMENT : regex2fragment e qi = (qf, frag))
+  (FRAGMENTS : TaggedENFA_FRAGMENTS frags rule topfrag)
+  (EPS_INCL : forall q, forall q', (q, q') ∈ frag.(frag_eps_edges) -> (q, q') ∈ topfrag.(frag_eps_edges))
+  (CHAR_INCL : forall edge, edge ∈ frag.(frag_char_edges) -> edge ∈ topfrag.(frag_char_edges))
+  : frag.(frag_accept) \in fragments_delta_star frags frag.(frag_start) s.
+Proof.
+  revert s IN_REGEX frags rule qi qf frag topfrag REGEX2FRAGMENT FRAGMENTS EPS_INCL CHAR_INCL.
+  induction e as [ | | c | e1 IH1 e2 IH2 | e1 IH1 e2 IH2 | e IH]; ii.
+  - simpl in IN_REGEX. contradiction.
+  - simpl in IN_REGEX. autorewrite with simplication_hints in IN_REGEX.
+    subst s. simpl in REGEX2FRAGMENT. inv REGEX2FRAGMENT.
+    pose proof (TaggedENFA_FRAGMENTS_delta_star_step frags rule topfrag FRAGMENTS) as [EPS _].
+    eapply EPS. eapply EPS_INCL. simpl. left. reflexivity.
+  - simpl in IN_REGEX. autorewrite with simplication_hints in IN_REGEX.
+    subst s. simpl in REGEX2FRAGMENT. inv REGEX2FRAGMENT.
+    pose proof (TaggedENFA_FRAGMENTS_delta_star_step frags rule topfrag FRAGMENTS) as [_ CHAR].
+    eapply CHAR with (edge := mkCharEdge qi c (qi + 1)).
+    eapply CHAR_INCL. simpl. left. reflexivity.
+  - simpl in REGEX2FRAGMENT. cbn [eval_regex] in IN_REGEX.
+    autorewrite with simplication_hints in IN_REGEX.
+    destruct (regex2fragment e1 (qi + 1)) as [qf1 frag1] eqn: REGEX1.
+    destruct (regex2fragment e2 (qf1 + 1)) as [qf2 frag2] eqn: REGEX2.
+    inv REGEX2FRAGMENT. destruct IN_REGEX as [IN1 | IN2].
+    + pose proof (TaggedENFA_FRAGMENTS_delta_star_step frags rule topfrag FRAGMENTS) as [EPS _].
+      pose proof (regex2fragment_start_accept _ _ _ _ REGEX1) as [START1 ACCEPT1].
+      rewrite <- app_nil_r with (l := s). eapply delta_star_app with (q2 := qf1).
+      * change s with ([] ++ s).
+        eapply delta_star_app with (q2 := qi + 1).
+        { eapply EPS. eapply EPS_INCL. simpl. left. reflexivity. }
+        { rewrite <- START1. rewrite <- ACCEPT1.
+          eapply IH1 with (s := s) (qi := qi + 1) (qf := qf1); eauto.
+          - intros q q' IN_EDGE. eapply EPS_INCL. simpl. s!; tauto.
+          - intros edge IN_EDGE. eapply CHAR_INCL. simpl. s!; tauto.
+        }
+      * eapply EPS. eapply EPS_INCL. simpl; s!; tauto.
+    + pose proof (TaggedENFA_FRAGMENTS_delta_star_step frags rule topfrag FRAGMENTS) as [EPS _].
+      pose proof (regex2fragment_start_accept _ _ _ _ REGEX2) as [START2 ACCEPT2].
+      rewrite <- app_nil_r with (l := s). eapply delta_star_app with (q2 := qf2).
+      * change s with ([] ++ s). eapply delta_star_app with (q2 := qf1 + 1).
+        { eapply EPS. eapply EPS_INCL. simpl. right; left. reflexivity. }
+        { rewrite <- START2. rewrite <- ACCEPT2.
+          eapply IH2 with (s := s) (qi := qf1 + 1) (qf := qf2); eauto.
+          - intros q q' IN_EDGE. eapply EPS_INCL. simpl. s!; tauto.
+          - intros edge IN_EDGE. eapply CHAR_INCL. simpl. s!; tauto.
+        }
+      * eapply EPS. eapply EPS_INCL. simpl. s!; tauto.
+  - simpl in REGEX2FRAGMENT. cbn [eval_regex] in IN_REGEX.
+    rewrite E.liftM2_spec in IN_REGEX.
+    destruct (regex2fragment e1 (qi + 1)) as [qf1 frag1] eqn: REGEX1.
+    destruct (regex2fragment e2 (qf1 + 1)) as [qf2 frag2] eqn: REGEX2.
+    inv REGEX2FRAGMENT.
+    destruct IN_REGEX as (s1 & IN1 & s2 & IN2 & EQ). subst s.
+    pose proof (TaggedENFA_FRAGMENTS_delta_star_step frags rule topfrag FRAGMENTS) as [EPS _].
+    pose proof (regex2fragment_start_accept _ _ _ _ REGEX1) as [START1 ACCEPT1].
+    pose proof (regex2fragment_start_accept _ _ _ _ REGEX2) as [START2 ACCEPT2].
+    eapply delta_star_app with (q2 := qf1) (s1 := s1) (s2 := s2).
+    + change s1 with ([] ++ s1).
+      eapply delta_star_app with (q2 := qi + 1).
+      { eapply EPS. eapply EPS_INCL. simpl. left. reflexivity. }
+      { rewrite <- START1. rewrite <- ACCEPT1.
+        eapply IH1 with (s := s1) (qi := qi + 1) (qf := qf1); eauto.
+        - intros q q' IN_EDGE. eapply EPS_INCL. simpl; s!; tauto.
+        - intros edge IN_EDGE. eapply CHAR_INCL. simpl; s!; tauto.
+      }
+    + rewrite <- app_nil_r with (l := s2).
+      eapply delta_star_app with (q2 := qf2).
+      * change s2 with ([] ++ s2).
+        eapply delta_star_app with (q2 := qf1 + 1).
+        { eapply EPS. eapply EPS_INCL. simpl. right; left. reflexivity. }
+        { rewrite <- START2. rewrite <- ACCEPT2.
+          eapply IH2 with (s := s2) (qi := qf1 + 1) (qf := qf2); eauto.
+          - intros q q' IN_EDGE. eapply EPS_INCL. simpl; s!; tauto.
+          - intros edge IN_EDGE. eapply CHAR_INCL. simpl; s!; tauto.
+        }
+      * eapply EPS. eapply EPS_INCL. simpl. s!; tauto.
+  - simpl in REGEX2FRAGMENT. simpl in IN_REGEX.
+    destruct (regex2fragment e (qi + 1)) as [qf1 frag1] eqn: REGEX1.
+    inv REGEX2FRAGMENT.
+    pose proof (TaggedENFA_FRAGMENTS_delta_star_step frags rule topfrag FRAGMENTS) as [EPS _].
+    pose proof (regex2fragment_start_accept _ _ _ _ REGEX1) as [START1 ACCEPT1].
+    assert (TAIL : forall t, t \in star (eval_regex e) -> qf1 + 1 \in fragments_delta_star frags (qi + 1) t).
+    { intros t STAR_IN. induction STAR_IN as [ | s1 s2 IN1 IN2 IHSTAR].
+      - eapply EPS. eapply EPS_INCL. simpl. right; right; left. reflexivity.
+      - replace (s1 ++ s2) with ((s1 ++ []) ++ s2) by now rewrite app_nil_r.
+        eapply delta_star_app with (q2 := qi + 1).
+        + eapply delta_star_app with (q2 := qf1).
+          * rewrite <- START1. rewrite <- ACCEPT1.
+            eapply IH with (s := s1) (qi := qi + 1) (qf := qf1); eauto.
+            { intros q q' IN_EDGE. eapply EPS_INCL. simpl. s!; tauto. }
+          * eapply EPS. eapply EPS_INCL. simpl. s!; tauto.
+        + exact IHSTAR.
+    }
+    change s with ([] ++ s).
+    eapply delta_star_app with (q2 := qi + 1).
+    + eapply EPS. eapply EPS_INCL. s!; tauto.
+    + eapply TAIL. exact IN_REGEX.
+Qed.
+
+Theorem regex2fragment_complete frags rule qi qf frag s
+  (REGEX2FRAGMENT : regex2fragment rule.(Rule.regex) qi = (qf, frag))
+  (FRAGMENTS : TaggedENFA_FRAGMENTS frags rule frag)
+  (IN_REGEX : s \in eval_regex rule.(Rule.regex))
+  : frag.(frag_accept) \in fragments_delta_star frags frag.(frag_start) s.
+Proof.
+  eapply regex2fragment_complete_aux; eauto.
+Qed.
+
+Theorem TaggedENFA_FRAGMENTS_complete qmax frags rule qi qf frag s
+  (REGEX2FRAGMENT : regex2fragment rule.(Rule.regex) qi = (qf, frag))
+  (FRAGMENTS : TaggedENFA_FRAGMENTS frags rule frag)
+  (IN_REGEX : s \in eval_regex rule.(Rule.regex))
+  : accepts (fragments2TaggedENFA qmax frags) s rule.(Rule.token).
+Proof.
+  destruct FRAGMENTS as [START ACCEPT EPS CHAR].
+  exists frag.(frag_accept). split; eauto.
+  change s with ([] ++ s).
+  eapply delta_star_app with (q2 := frag.(frag_start)).
+  - eapply delta_star_eps with (q1 := frag.(frag_start)); eauto. econs.
+  - eapply regex2fragment_complete; eauto. econs; eauto.
+Qed.
+
+Theorem rules2fragments_complete qi rules qmax frags rule
+  (FRAGS : rules2fragments qi rules = (qmax, frags))
+  (IN_RULE : rule ∈ rules)
+  : exists qi_rule, exists qf, exists frag, regex2fragment rule.(Rule.regex) qi_rule = (qf, frag) /\ (rule, frag) ∈ frags.
+Proof.
+  revert qi qmax frags FRAGS IN_RULE. induction rules as [ | rule' rules IH]; intros qi qmax frags FRAGS IN_RULE; simpl in IN_RULE; try tauto.
+  simpl in FRAGS. destruct (regex2fragment rule'.(Rule.regex) qi) as [qf frag] eqn: REGEX2FRAGMENT.
+  destruct (rules2fragments (qf + 1) rules) as [qmax' frags'] eqn: FRAGS'. s!; des; subst.
+  - exists qi, qf, frag. ss!.
+  - pose proof (IH (qf + 1) qmax frags' FRAGS' IN_RULE) as (qi_rule & qf_rule & frag_rule & REGEX & IN_FRAGS).
+    exists qi_rule, qf_rule, frag_rule. ss!.
+Qed.
+
+Lemma rules2fragments_sound qi rules qmax frags rule frag
+  (FRAGS : rules2fragments qi rules = (qmax, frags))
+  (IN_FRAG : (rule, frag) ∈ frags)
+  : rule ∈ rules.
+Proof.
+  revert qi qmax frags FRAGS IN_FRAG. induction rules as [ | rule' rules IH]; ii; simpl in FRAGS.
+  - now inv FRAGS.
+  - destruct (regex2fragment rule'.(Rule.regex) qi) as [qf frag'] eqn: REGEX.
+    destruct (rules2fragments (qf + 1) rules) as [qmax' frags'] eqn: FRAGS'.
+    s!; des; subst. destruct IN_FRAG as [EQ | IN_FRAG]; ss!.
+Qed.
+
+Lemma rules2fragments_bounds qi rules qmax frags
+  (FRAGS : rules2fragments qi rules = (qmax, frags))
+  : qi <= qmax /\ ⟪ BOUND : forall rule, forall frag, (rule, frag) ∈ frags -> (exists qi_rule, exists qf, regex2fragment rule.(Rule.regex) qi_rule = (qf, frag) /\ FRAGMENT_BOUNDS qi_rule qf frag /\ qi <= qi_rule /\ qf < qmax) ⟫.
+Proof.
+  revert qi qmax frags FRAGS.
+  induction rules as [ | rule' rules IH]; intros qi qmax frags FRAGS; simpl in FRAGS.
+  - inv FRAGS. split; [lia | intros rule frag IN; contradiction].
+  - destruct (regex2fragment rule'.(Rule.regex) qi) as [qf frag] eqn: REGEX2FRAGMENT.
+    destruct (rules2fragments (qf + 1) rules) as [qmax' frags'] eqn: FRAGS'.
+    injection FRAGS as Hqmax Hfrags. subst qmax frags.
+    pose proof (regex2fragment_bounds _ _ _ _ REGEX2FRAGMENT) as BOUNDS.
+    assert (LT : qi < qf) by now destruct BOUNDS as [_ _ LT _ _].
+    pose proof (IH (qf + 1) qmax' frags' FRAGS') as [QMAX TAIL].
+    split; [done! | intros rule frag' IN]. destruct IN as [EQ | IN].
+    + inv EQ. exists qi, qf. split; eauto. split; eauto. split; lia.
+    + pose proof (TAIL rule frag' IN) as (qi_rule & qf_rule & REGEX & BOUNDS' & LE_START & LT_END).
+      exists qi_rule, qf_rule; done!.
+Qed.
+
+Lemma rules2fragments_ranges_disjoint qi rules qmax frags rule1 frag1 qi1 qf1 rule2 frag2 qi2 qf2 q
+  (FRAGS : rules2fragments qi rules = (qmax, frags))
+  (IN1 : (rule1, frag1) ∈ frags)
+  (IN2 : (rule2, frag2) ∈ frags)
+  (REGEX1 : regex2fragment rule1.(Rule.regex) qi1 = (qf1, frag1))
+  (REGEX2 : regex2fragment rule2.(Rule.regex) qi2 = (qf2, frag2))
+  (RANGE1 : qi1 <= q <= qf1)
+  (RANGE2 : qi2 <= q <= qf2)
+  : (rule1, frag1) = (rule2, frag2).
+Proof.
+  revert qi qmax frags FRAGS rule1 frag1 qi1 qf1 rule2 frag2 qi2 qf2 q IN1 IN2 REGEX1 REGEX2 RANGE1 RANGE2. induction rules as [ | rule rules IH]; ii; simpl in FRAGS.
+  - now inv FRAGS.
+  - destruct (regex2fragment rule.(Rule.regex) qi) as [qf frag] eqn: REGEX.
+    destruct (rules2fragments (qf + 1) rules) as [qmax' frags'] eqn: FRAGS'.
+    s!; des; subst. pose proof (rules2fragments_bounds _ _ _ _ FRAGS') as [_ TAIL_BOUNDS].
+    destruct IN1 as [EQ1 | IN1]; destruct IN2 as [EQ2 | IN2]; rewrite <- inject_pair_eq.
+    + inv EQ1. inv EQ2. reflexivity.
+    + inv EQ1.
+      pose proof (regex2fragment_same_fragment _ _ _ _ _ _ REGEX1 REGEX) as [EQ_QI EQ_QF]. subst qi1 qf1.
+      pose proof (TAIL_BOUNDS _ _ IN2) as (qi2' & qf2' & REGEX2' & _ & LE2 & _).
+      pose proof (regex2fragment_same_fragment _ _ _ _ _ _ REGEX2 REGEX2') as [EQ_QI EQ_QF]. subst qi2 qf2.
+      lia.
+    + inv EQ2.
+      pose proof (regex2fragment_same_fragment _ _ _ _ _ _ REGEX2 REGEX) as [EQ_QI EQ_QF]. subst qi2 qf2.
+      pose proof (TAIL_BOUNDS _ _ IN1) as (qi1' & qf1' & REGEX1' & _ & LE1 & _).
+      pose proof (regex2fragment_same_fragment _ _ _ _ _ _ REGEX1 REGEX1') as [EQ_QI EQ_QF]. subst qi1 qf1.
+      lia.
+    + eapply IH; eauto.
+Qed.
+
+#[local] Hint Resolve regex2fragment_bounds : simplication_hints.
+
+Lemma fragment_eps_edges_owner qi rules qmax frags q q'
+  (FRAGS : rules2fragments qi rules = (qmax, frags))
+  (IN_EDGE : (q, q') ∈ fragment_eps_edges frags)
+  (SRC_NONZERO : q ≠ 0)
+  : exists rule, exists frag, exists qi_rule, exists qf, (rule, frag) ∈ frags /\ regex2fragment rule.(Rule.regex) qi_rule = (qf, frag) /\ FRAGMENT_BOUNDS qi_rule qf frag /\ qi <= qi_rule /\ qf < qmax /\ qi_rule <= q <= qf /\ (q, q') ∈ frag.(frag_eps_edges).
+Proof.
+  revert qi qmax frags FRAGS IN_EDGE; induction rules as [ | rule rules IH]; ii; simpl in FRAGS.
+  - now inv FRAGS.
+  - destruct (regex2fragment rule.(Rule.regex) qi) as [qf frag] eqn: REGEX.
+    destruct (rules2fragments (qf + 1) rules) as [qmax' frags'] eqn: FRAGS'.
+    s!; des; subst. pose proof (rules2fragments_bounds _ _ _ _ FRAGS') as [QMAX _].
+    simpl in IN_EDGE. destruct IN_EDGE as [EQ | IN_EDGE].
+    + now inv EQ.
+    + rewrite in_app_iff in IN_EDGE. destruct IN_EDGE as [IN_EDGE | IN_EDGE].
+      * pose proof (regex2fragment_bounds _ _ _ _ REGEX) as [_ _ LT EPS _].
+        pose proof (EPS _ IN_EDGE). unfold eps_edge_in_range in *. simpl in *.
+        exists rule, frag, qi, qf. splits; lia || ss!.
+      * pose proof (regex2fragment_bounds _ _ _ _ REGEX) as [_ _ LT _ _].
+        pose proof (IH (qf + 1) qmax frags' FRAGS' IN_EDGE) as (rule' & frag' & qi_rule & qf' & IN_FRAG & REGEX' & BOUNDS & LE & LT' & RANGE & IN_EDGE').
+        exists rule', frag', qi_rule, qf'. splits; lia || ss!.
+Qed.
+
+Lemma fragment_eps_edges_start_sound qi rules qmax frags q'
+  (FRAGS : rules2fragments qi rules = (qmax, frags))
+  (qi_POS : 0 < qi)
+  (IN_EDGE : (0, q') ∈ fragment_eps_edges frags)
+  : exists rule, exists frag, exists qi_rule, exists qf, (rule, frag) ∈ frags /\ regex2fragment rule.(Rule.regex) qi_rule = (qf, frag) /\ q' = frag.(frag_start).
+Proof.
+  revert qi qmax frags q' FRAGS qi_POS IN_EDGE; induction rules as [ | rule rules IH]; ii; simpl in FRAGS.
+  - now inv FRAGS.
+  - destruct (regex2fragment rule.(Rule.regex) qi) as [qf frag] eqn: REGEX.
+    destruct (rules2fragments (qf + 1) rules) as [qmax' frags'] eqn: FRAGS'.
+    s!; des; subst. simpl in IN_EDGE. destruct IN_EDGE as [EQ | IN_EDGE].
+    + inv EQ. exists rule, frag, qi, qf. ss!.
+    + s!. destruct IN_EDGE as [IN_EDGE | IN_EDGE].
+      * pose proof (regex2fragment_bounds _ _ _ _ REGEX) as [_ _ _ EPS _].
+        pose proof (EPS _ IN_EDGE); done!.
+      * pose proof (regex2fragment_bounds _ _ _ _ REGEX) as [_ _ LT _ _].
+        assert (qi_POS' : 0 < qf + 1) by lia.
+        pose proof (IH (qf + 1) qmax frags' q' FRAGS' qi_POS' IN_EDGE) as (rule' & frag' & qi_rule & qf' & IN_FRAG & REGEX' & START).
+        exists rule', frag', qi_rule, qf'. done!.
+Qed.
+
+Lemma fragment_char_edges_owner qi rules qmax frags edge
+  (FRAGS : rules2fragments qi rules = (qmax, frags))
+  (IN_EDGE : edge ∈ fragment_char_edges frags)
+  : exists rule, exists frag, exists qi_rule, exists qf, (rule, frag) ∈ frags /\ regex2fragment rule.(Rule.regex) qi_rule = (qf, frag) /\ FRAGMENT_BOUNDS qi_rule qf frag /\ qi <= qi_rule /\ qf < qmax /\ qi_rule <= edge.(char_edge_src) <= qf /\ edge ∈ frag.(frag_char_edges).
+Proof.
+  revert qi qmax frags FRAGS IN_EDGE; induction rules as [ | rule rules IH]; ii; simpl in FRAGS.
+  - now inv FRAGS.
+  - destruct (regex2fragment rule.(Rule.regex) qi) as [qf frag] eqn: REGEX.
+    destruct (rules2fragments (qf + 1) rules) as [qmax' frags'] eqn: FRAGS'.
+    s!; des; subst. pose proof (rules2fragments_bounds _ _ _ _ FRAGS') as [QMAX _].
+    simpl in IN_EDGE. rewrite in_app_iff in IN_EDGE. destruct IN_EDGE as [IN_EDGE | IN_EDGE].
+    + pose proof (regex2fragment_bounds _ _ _ _ REGEX) as BOUNDS.
+      destruct BOUNDS as [_ _ LT _ CHAR].
+      pose proof (CHAR _ IN_EDGE). unfold char_edge_in_range in *.
+      exists rule, frag, qi, qf. splits; lia || ss!.
+    + pose proof (regex2fragment_bounds _ _ _ _ REGEX) as [_ _ LT _ _].
+      pose proof (IH (qf + 1) qmax frags' FRAGS' IN_EDGE) as (rule' & frag' & qi_rule & qf' & IN_FRAG & REGEX' & BOUNDS & LE & LT' & RANGE & IN_EDGE').
+      exists rule', frag', qi_rule, qf'. splits; lia || ss!.
+Qed.
+
+Lemma fragments2TaggedENFA_okay rules qmax frags
+  (FRAGS : rules2fragments 1 rules = (qmax, frags))
+  : TaggedENFA.okay (fragments2TaggedENFA qmax frags).
+Proof.
+  split; simpl.
+  - rewrite in_seq. pose proof (rules2fragments_bounds _ _ _ _ FRAGS) as [LE _]. lia.
+  - intros q tag ACCEPT.
+    pose proof (fragment_accept_states_sound _ _ _ ACCEPT) as (rule & frag & IN_FRAG & ACCEPT_EQ & TOKEN_EQ); subst q tag.
+    pose proof (rules2fragments_bounds _ _ _ _ FRAGS) as [_ BOUND].
+    pose proof (BOUND _ _ IN_FRAG) as (qi_rule & qf & REGEX & [_ ACCEPT_EQ _ _ _] & LE_START & LT_END); subst qf.
+    rewrite in_seq. lia.
+  - intros q q' IN_STATES STEP.
+    pose proof (eps_step_from_edges_sound _ _ _ STEP) as IN_EDGE.
+    destruct (eq_dec q 0) as [EQ | NE].
+    + subst q.
+      assert (QI_POS : 0 < 1) by lia.
+      pose proof (fragment_eps_edges_start_sound _ _ _ _ _ FRAGS QI_POS IN_EDGE) as (rule & frag & qi_rule & qf & IN_FRAG & REGEX & START_EQ); subst q'.
+      pose proof (rules2fragments_bounds _ _ _ _ FRAGS) as [_ BOUND].
+      pose proof (BOUND _ _ IN_FRAG) as (qi_rule' & qf' & REGEX' & [START_EQ _ LT _ _] & LE_START & LT_END).
+      pose proof (regex2fragment_same_fragment _ _ _ _ _ _ REGEX REGEX') as [EQ_QI EQ_QF]; subst qi_rule' qf'.
+      rewrite in_seq. lia.
+    + pose proof (fragment_eps_edges_owner _ _ _ _ _ _ FRAGS IN_EDGE NE) as (rule & frag & qi_rule & qf & IN_FRAG & REGEX & [_ _ _ EPS _] & LE_START & LT_END & RANGE & IN_EDGE').
+      pose proof (EPS _ IN_EDGE') as RANGE'.
+      unfold eps_edge_in_range in RANGE'. simpl in RANGE'. rewrite in_seq. lia.
+  - intros q q' c IN_STATES STEP.
+    pose proof (char_step_from_edges_sound _ _ _ _ STEP) as (edge & IN_EDGE & SRC & LABEL & DST); subst q q' c.
+    pose proof (fragment_char_edges_owner _ _ _ _ _ FRAGS IN_EDGE) as (rule & frag & qi_rule & qf & IN_FRAG & REGEX & BOUNDS & LE_START & LT_END & RANGE & IN_EDGE').
+    destruct BOUNDS as [_ _ _ _ CHAR].
+    pose proof (CHAR _ IN_EDGE') as RANGE'.
+    unfold char_edge_in_range in RANGE'. simpl in RANGE'. rewrite in_seq. lia.
+Qed.
+
+Theorem mkUnitedTaggedENFA_okay rules
+  : TaggedENFA.okay (mkUnitedTaggedENFA rules).
+Proof.
+  unfold mkUnitedTaggedENFA. destruct (rules2fragments 1 rules) as [qmax frags] eqn: FRAGS.
+  now eapply fragments2TaggedENFA_okay with (rules := rules).
+Qed.
+
+Lemma fragment_eps_edges_isolate qi rules qmax frags rule frag qi_rule qf q q'
+  (FRAGS : rules2fragments qi rules = (qmax, frags))
+  (IN_FRAG : (rule, frag) ∈ frags)
+  (REGEX : regex2fragment rule.(Rule.regex) qi_rule = (qf, frag))
+  (SRC_NONZERO : q ≠ 0)
+  (RANGE : qi_rule <= q <= qf)
+  (IN_EDGE : (q, q') ∈ fragment_eps_edges frags)
+  : (q, q') ∈ frag.(frag_eps_edges).
+Proof.
+  pose proof (fragment_eps_edges_owner _ _ _ _ _ _ FRAGS IN_EDGE SRC_NONZERO) as (rule' & frag' & qi_rule' & qf' & IN_FRAG' & REGEX' & _ & _ & _ & RANGE' & IN_EDGE').
+  pose proof (rules2fragments_ranges_disjoint _ _ _ _ _ _ _ _ _ _ _ _ _ FRAGS IN_FRAG IN_FRAG' REGEX REGEX' RANGE RANGE') as EQ.
+  ss!.
+Qed.
+
+Lemma fragment_char_edges_isolate qi rules qmax frags rule frag qi_rule qf edge
+  (FRAGS : rules2fragments qi rules = (qmax, frags))
+  (IN_FRAG : (rule, frag) ∈ frags)
+  (REGEX : regex2fragment rule.(Rule.regex) qi_rule = (qf, frag))
+  (RANGE : qi_rule <= edge.(char_edge_src) <= qf)
+  (IN_EDGE : edge ∈ fragment_char_edges frags)
+  : edge ∈ frag.(frag_char_edges).
+Proof.
+  pose proof (fragment_char_edges_owner _ _ _ _ _ FRAGS IN_EDGE) as (rule' & frag' & qi_rule' & qf' & IN_FRAG' & REGEX' & _ & _ & _ & RANGE' & IN_EDGE').
+  pose proof (rules2fragments_ranges_disjoint _ _ _ _ _ _ _ _ _ _ _ _ _ FRAGS IN_FRAG IN_FRAG' REGEX REGEX' RANGE RANGE') as EQ.
+  ss!.
+Qed.
+
+Lemma rules2fragments_start_ge qi rules qmax frags rule frag qi_rule qf
+  (FRAGS : rules2fragments qi rules = (qmax, frags))
+  (IN_FRAG : (rule, frag) ∈ frags)
+  (REGEX : regex2fragment rule.(Rule.regex) qi_rule = (qf, frag))
+  : qi <= qi_rule.
+Proof.
+  pose proof (rules2fragments_bounds _ _ _ _ FRAGS) as [_ BOUND].
+  pose proof (BOUND _ _ IN_FRAG) as (qi_rule' & qf' & REGEX' & _ & LE & _).
+  pose proof (regex2fragment_same_fragment _ _ _ _ _ _ REGEX REGEX') as [EQ _].
+  ss!.
+Qed.
+
+Lemma delta_star_fragment_range qi rules qmax frags rule frag qi_rule qf q q' s
+  (FRAGS : rules2fragments qi rules = (qmax, frags))
+  (IN_FRAG : (rule, frag) ∈ frags)
+  (REGEX : regex2fragment rule.(Rule.regex) qi_rule = (qf, frag))
+  (qi_POS : 0 < qi)
+  (RANGE : qi_rule <= q <= qf)
+  (DELTA : q' \in fragments_delta_star frags q s)
+  : qi_rule <= q' <= qf.
+Proof.
+  revert qi rules rule frag qi_rule qf FRAGS IN_FRAG REGEX qi_POS RANGE; induction DELTA; ii.
+  - exact RANGE.
+  - pose proof (eps_step_from_edges_sound _ _ _ STEP) as IN_EDGE.
+    assert (SRC_NONZERO : q ≠ 0) by (pose proof (rules2fragments_start_ge _ _ _ _ _ _ _ _ FRAGS IN_FRAG REGEX); lia).
+    pose proof (fragment_eps_edges_isolate _ _ _ _ _ _ _ _ _ _ FRAGS IN_FRAG REGEX SRC_NONZERO RANGE IN_EDGE) as IN_FRAG_EDGE.
+    pose proof (regex2fragment_bounds _ _ _ _ REGEX) as [_ _ _ EPS _].
+    pose proof (EPS _ IN_FRAG_EDGE). unfold eps_edge_in_range in *. simpl in *.
+    eapply IHDELTA; eauto. lia.
+  - pose proof (char_step_from_edges_sound _ _ _ _ STEP) as (edge & IN_EDGE & SRC & LABEL & DST).
+    assert (RANGE_SRC : qi_rule <= edge.(char_edge_src) <= qf) by lia.
+    pose proof (fragment_char_edges_isolate _ _ _ _ _ _ _ _ _ FRAGS IN_FRAG REGEX RANGE_SRC IN_EDGE) as IN_FRAG_EDGE.
+    pose proof (regex2fragment_bounds _ _ _ _ REGEX) as [_ _ _ _ CHAR].
+    pose proof (CHAR _ IN_FRAG_EDGE). unfold char_edge_in_range in *.
+    eapply IHDELTA; eauto. lia.
+Qed.
+
+Lemma delta_star_global_to_fragment qi rules qmax frags rule frag qi_rule qf q q' s
+  (FRAGS : rules2fragments qi rules = (qmax, frags))
+  (IN_FRAG : (rule, frag) ∈ frags)
+  (REGEX : regex2fragment rule.(Rule.regex) qi_rule = (qf, frag))
+  (qi_POS : 0 < qi)
+  (RANGE : qi_rule <= q <= qf)
+  (DELTA : q' \in fragments_delta_star frags q s)
+  : q' \in fragment_delta_star frag q s.
+Proof.
+  revert qi rules rule frag qi_rule qf FRAGS IN_FRAG REGEX qi_POS RANGE. induction DELTA; ii.
+  - econs.
+  - pose proof (eps_step_from_edges_sound _ _ _ STEP) as IN_EDGE.
+    assert (SRC_NONZERO : q ≠ 0) by (pose proof (rules2fragments_start_ge _ _ _ _ _ _ _ _ FRAGS IN_FRAG REGEX); lia).
+    pose proof (fragment_eps_edges_isolate _ _ _ _ _ _ _ _ _ _ FRAGS IN_FRAG REGEX SRC_NONZERO RANGE IN_EDGE) as IN_FRAG_EDGE.
+    pose proof (regex2fragment_bounds _ _ _ _ REGEX) as [_ _ _ EPS _].
+    pose proof (EPS _ IN_FRAG_EDGE). unfold eps_edge_in_range in *. simpl in *.
+    eapply delta_star_eps.
+    + eapply eps_step_from_edges_complete. exact IN_FRAG_EDGE.
+    + eapply IHDELTA; eauto. lia.
+  - pose proof (char_step_from_edges_sound _ _ _ _ STEP) as (edge & IN_EDGE & SRC & LABEL & DST).
+    assert (RANGE_SRC : qi_rule <= edge.(char_edge_src) <= qf) by lia.
+    pose proof (fragment_char_edges_isolate _ _ _ _ _ _ _ _ _ FRAGS IN_FRAG REGEX RANGE_SRC IN_EDGE) as IN_FRAG_EDGE.
+    pose proof (regex2fragment_bounds _ _ _ _ REGEX) as [_ _ _ _ CHAR].
+    pose proof (CHAR _ IN_FRAG_EDGE). unfold char_edge_in_range in *.
+    eapply delta_star_char with (q1 := edge.(char_edge_dst)).
+    + rewrite <- SRC. rewrite <- LABEL. eapply char_step_from_edges_complete. exact IN_FRAG_EDGE.
+    + rewrite DST. eapply IHDELTA; eauto. lia.
+Qed.
+
+Lemma regex2fragment_global_to_local qi rules qmax frags rule qf frag s
+  (FRAGS : rules2fragments qi rules = (qmax, frags))
+  (IN_FRAG : (rule, frag) ∈ frags)
+  (REGEX : regex2fragment rule.(Rule.regex) frag.(frag_start) = (qf, frag))
+  (qi_POS : 0 < qi)
+  (DELTA : frag.(frag_accept) \in fragments_delta_star frags frag.(frag_start) s)
+  : frag.(frag_accept) \in fragment_delta_star frag frag.(frag_start) s.
+Proof.
+  pose proof (regex2fragment_bounds _ _ _ _ REGEX) as [START ACCEPT LT _ _].
+  eapply delta_star_global_to_fragment; eauto. lia.
+Qed.
+
+Lemma delta_star_fragment_elim qi rules qmax frags rule frag qi_rule qf q q' s
+  (FRAGS : rules2fragments qi rules = (qmax, frags))
+  (IN_FRAG : (rule, frag) ∈ frags)
+  (REGEX : regex2fragment rule.(Rule.regex) qi_rule = (qf, frag))
+  (qi_POS : 0 < qi)
+  (RANGE : qi_rule <= q <= qf)
+  (DELTA : q' \in fragments_delta_star frags q s)
+  : ⟪ DELTA_STAR_NIL : s = [] /\ q' = q ⟫ \/ ⟪ DELTA_STAR_EPS : exists q1, (q, q1) ∈ frag.(frag_eps_edges) /\ q' \in fragments_delta_star frags q1 s ⟫ \/ ⟪ DELTA_STAR_CHAR : exists edge, exists s', s = edge.(char_edge_label) :: s' /\ edge ∈ frag.(frag_char_edges) /\ q' \in fragments_delta_star frags edge.(char_edge_dst) s' ⟫.
+Proof.
+  pose proof (delta_star_elim _ _ q q' s DELTA) as [NIL | [EPS | CHAR]]; [left | right; left | right; right]; unnw; try tauto.
+  - destruct EPS as (q1 & STEP & REST).
+    pose proof (eps_step_from_edges_sound _ _ _ STEP) as IN_EDGE.
+    assert (SRC_NONZERO : q ≠ 0) by now pose proof (rules2fragments_start_ge _ _ _ _ _ _ _ _ FRAGS IN_FRAG REGEX); lia.
+    pose proof (fragment_eps_edges_isolate _ _ _ _ _ _ _ _ _ _ FRAGS IN_FRAG REGEX SRC_NONZERO RANGE IN_EDGE) as IN_FRAG_EDGE.
+    exists q1. ss!.
+  - destruct CHAR as (c & s' & q1 & EQ & STEP & REST).
+    pose proof (char_step_from_edges_sound _ _ _ _ STEP) as (edge & IN_EDGE & SRC & LABEL & DST).
+    assert (RANGE_SRC : qi_rule <= edge.(char_edge_src) <= qf) by lia.
+    pose proof (fragment_char_edges_isolate _ _ _ _ _ _ _ _ _ FRAGS IN_FRAG REGEX RANGE_SRC IN_EDGE) as IN_FRAG_EDGE.
+    exists edge, s'. ss!.
+Qed.
+
+Lemma fragment_delta_star_elim frag q q' s
+  (DELTA : q' \in fragment_delta_star frag q s)
+  : ⟪ DELTA_STAR_NIL : s = [] /\ q' = q ⟫ \/ ⟪ DELTA_STAR_EPS : exists q1, (q, q1) ∈ frag.(frag_eps_edges) /\ q' \in fragment_delta_star frag q1 s ⟫ \/ ⟪ DELTA_STAR_CHAR : exists edge, exists s', s = edge.(char_edge_label) :: s' /\ edge ∈ frag.(frag_char_edges) /\ q' \in fragment_delta_star frag edge.(char_edge_dst) s' ⟫.
+Proof.
+  pose proof (delta_star_elim _ _ q q' s DELTA) as [NIL | [EPS | CHAR]]; [left | right; left | right; right]; unnw; try tauto.
+  - destruct EPS as (q1 & STEP & REST). pose proof (eps_step_from_edges_sound _ _ _ STEP). exists q1; ss!.
+  - destruct CHAR as (c & s' & q1 & EQ & STEP & REST). pose proof (char_step_from_edges_sound _ _ _ _ STEP) as (edge & IN_EDGE & SRC & LABEL & DST). exists edge, s'; ss!.
+Qed.
+
+Lemma fragment_delta_star_elim_with_src frag q q' s
+  (DELTA : q' \in fragment_delta_star frag q s)
+  : ⟪ DELTA_STAR_NIL : s = [] /\ q' = q ⟫ \/ ⟪ DELTA_STAR_EPS : exists q1, (q, q1) ∈ frag.(frag_eps_edges) /\ q' \in fragment_delta_star frag q1 s ⟫ \/ ⟪ DELTA_STAR_CHAR : exists edge, exists s', s = edge.(char_edge_label) :: s' /\ edge.(char_edge_src) = q /\ edge ∈ frag.(frag_char_edges) /\ q' \in fragment_delta_star frag edge.(char_edge_dst) s' ⟫.
+Proof.
+  pose proof (delta_star_elim _ _ q q' s DELTA) as [NIL | [EPS | CHAR]]; [left | right; left | right; right]; unnw; try tauto.
+  - destruct EPS as (q1 & STEP & REST). pose proof (eps_step_from_edges_sound _ _ _ STEP). exists q1; ss!.
+  - destruct CHAR as (c & s' & q1 & EQ & STEP & REST). pose proof (char_step_from_edges_sound _ _ _ _ STEP) as (edge & IN_EDGE & SRC & LABEL & DST). exists edge, s'. ss!.
+Qed.
+
+Lemma regex2fragment_Union_delta_star_start qi qf frag e1 e2 s
+  (REGEX : regex2fragment (Re.Union e1 e2) qi = (qf, frag))
+  (DELTA : frag.(frag_accept) \in fragment_delta_star frag frag.(frag_start) s)
+  : exists qf1, exists frag1, exists qf2, exists frag2, regex2fragment e1 (qi + 1) = (qf1, frag1) /\ regex2fragment e2 (qf1 + 1) = (qf2, frag2) /\ (frag.(frag_accept) \in fragment_delta_star frag (qi + 1) s \/ frag.(frag_accept) \in fragment_delta_star frag (qf1 + 1) s).
+Proof.
+  simpl in REGEX. destruct (regex2fragment e1 (qi + 1)) as [qf1 frag1] eqn: REGEX1. destruct (regex2fragment e2 (qf1 + 1)) as [qf2 frag2] eqn: REGEX2. inv REGEX.
+  exists qf1, frag1, qf2, frag2. splits; simpl; eauto.
+  pose proof (regex2fragment_bounds _ _ _ _ REGEX1) as [_ _ LT1 EPS1 CHAR1].
+  pose proof (regex2fragment_bounds _ _ _ _ REGEX2) as [_ _ LT2 EPS2 CHAR2].
+  pose proof (fragment_delta_star_elim_with_src _ _ _ _ DELTA) as [NIL | [EPS | CHAR]].
+  - des; simpl in *; lia.
+  - destruct EPS as (q1 & IN_EDGE & REST). simpl in IN_EDGE. s!; des; subst.
+    + left. exact REST.
+    + right. exact REST.
+    + exfalso; lia.
+    + exfalso; lia.
+    + pose proof (EPS1 _ IN_EDGE). unfold eps_edge_in_range in *. simpl in *. exfalso; lia.
+    + pose proof (EPS2 _ IN_EDGE). unfold eps_edge_in_range in *. simpl in *. exfalso; lia.
+  - destruct CHAR as (edge & s' & EQ & SRC & IN_EDGE & REST). simpl in IN_EDGE. s!; des.
+    + pose proof (CHAR1 _ IN_EDGE) as [[SRC_LO SRC_HI] _]. exfalso; lia.
+    + pose proof (CHAR2 _ IN_EDGE) as [[SRC_LO SRC_HI] _]. exfalso; lia.
+Qed.
+
+#[local] Opaque eps_step_from_edges.
+#[local] Opaque char_step_from_edges.
+
+#[local] Hint Constructors eclosure : simplication_hints.
+#[local] Hint Constructors delta_star : simplication_hints.
+
+Lemma regex2fragment_Union_left_delta_star_split qi qf frag e1 e2 qf1 frag1 qf2 frag2 q q' s
+  (REGEX : regex2fragment (Re.Union e1 e2) qi = (qf, frag))
+  (REGEX1 : regex2fragment e1 (qi + 1) = (qf1, frag1))
+  (REGEX2 : regex2fragment e2 (qf1 + 1) = (qf2, frag2))
+  (RANGE : qi + 1 <= q <= qf1)
+  (DELTA : q' \in fragment_delta_star frag q s)
+  (ACCEPT : q' = frag.(frag_accept))
+  : exists s1, exists s2, s = s1 ++ s2 /\ qf1 \in fragment_delta_star frag1 q s1 /\ frag.(frag_accept) \in fragment_delta_star frag frag.(frag_accept) s2.
+Proof.
+  revert q q' s RANGE DELTA ACCEPT; simpl in REGEX; rewrite -> REGEX1, -> REGEX2 in REGEX; inv REGEX.
+  intros q q' s RANGE DELTA ACCEPT.
+  pose proof (regex2fragment_bounds _ _ _ _ REGEX1) as [_ _ LT1 EPS1 CHAR1].
+  pose proof (regex2fragment_bounds _ _ _ _ REGEX2) as [_ _ LT2 EPS2 CHAR2].
+  induction DELTA.
+  - simpl in *. exfalso; lia.
+  - pose proof (eps_step_from_edges_sound _ _ _ STEP) as IN_EDGE. simpl in IN_EDGE; s!; des; subst.
+    + exfalso; lia.
+    + exfalso; lia.
+    + exists [], s; ss!.
+    + exfalso; lia.
+    + pose proof (EPS1 _ IN_EDGE) as [[SRC_LO SRC_HI] [DST_LO DST_HI]]. simpl in SRC_LO, SRC_HI, DST_LO, DST_HI.
+      assert (RANGE_STEP : qi + 1 <= q1 <= qf1) by lia.
+      pose proof (IHDELTA RANGE_STEP eq_refl) as (s1 & s2 & EQ & DELTA1 & DELTA2).
+      exists s1, s2. splits; eauto. eapply delta_star_eps; eauto. eapply eps_step_from_edges_complete; eauto.
+    + pose proof (EPS2 _ IN_EDGE) as [[SRC_LO SRC_HI] _]. simpl in *. lia.
+  - pose proof (char_step_from_edges_sound _ _ _ _ STEP) as (edge & IN_EDGE & SRC & LABEL & DST); simpl in IN_EDGE; s!; des.
+    + pose proof (CHAR1 _ IN_EDGE) as [[SRC_LO SRC_HI] [DST_LO DST_HI]].
+      assert (RANGE_STEP : qi + 1 <= q1 <= qf1) by lia.
+      pose proof (IHDELTA RANGE_STEP ACCEPT) as (s1 & s2 & EQ & DELTA1 & DELTA2).
+      exists (edge.(char_edge_label) :: s1), s2. splits; auto.
+      * rewrite EQ. simpl. now rewrite LABEL.
+      * eapply delta_star_char with (q1 := q1); auto.
+        rewrite <- DST. rewrite <- SRC. eapply char_step_from_edges_complete; auto.
+    + pose proof (CHAR2 _ IN_EDGE) as [[SRC_LO SRC_HI] _]. simpl in SRC. lia.
+Qed.
+
+Lemma regex2fragment_Union_right_delta_star_split qi qf frag e1 e2 qf1 frag1 qf2 frag2 q q' s
+  (REGEX : regex2fragment (Re.Union e1 e2) qi = (qf, frag))
+  (REGEX1 : regex2fragment e1 (qi + 1) = (qf1, frag1))
+  (REGEX2 : regex2fragment e2 (qf1 + 1) = (qf2, frag2))
+  (RANGE : qf1 + 1 <= q <= qf2)
+  (DELTA : q' \in fragment_delta_star frag q s)
+  (ACCEPT : q' = frag.(frag_accept))
+  : exists s1, exists s2, s = s1 ++ s2 /\ qf2 \in fragment_delta_star frag2 q s1 /\ frag.(frag_accept) \in fragment_delta_star frag frag.(frag_accept) s2.
+Proof.
+  revert q q' s RANGE DELTA ACCEPT; simpl in REGEX. rewrite -> REGEX1, -> REGEX2 in REGEX. inv REGEX; ii.
+  pose proof (regex2fragment_bounds _ _ _ _ REGEX1) as [_ _ LT1 EPS1 CHAR1].
+  pose proof (regex2fragment_bounds _ _ _ _ REGEX2) as [_ _ LT2 EPS2 CHAR2].
+  induction DELTA.
+  - simpl in *. exfalso; lia.
+  - pose proof (eps_step_from_edges_sound _ _ _ STEP) as IN_EDGE. simpl in IN_EDGE; s!; des; subst.
+    + exfalso; lia.
+    + exfalso; lia.
+    + exfalso; lia.
+    + exists [], s; ss!.
+    + pose proof (EPS1 _ IN_EDGE) as [[SRC_LO SRC_HI] _]. simpl in *. lia.
+    + pose proof (EPS2 _ IN_EDGE) as [[SRC_LO SRC_HI] [DST_LO DST_HI]].
+      simpl in SRC_LO, SRC_HI, DST_LO, DST_HI.
+      assert (RANGE_STEP : qf1 + 1 <= q1 <= qf2) by lia.
+      pose proof (IHDELTA RANGE_STEP eq_refl) as (s1 & s2 & EQ & DELTA1 & DELTA2).
+      exists s1, s2. splits; eauto. eapply delta_star_eps; eauto. eapply eps_step_from_edges_complete; eauto.
+  - pose proof (char_step_from_edges_sound _ _ _ _ STEP) as (edge & IN_EDGE & SRC & LABEL & DST); simpl in IN_EDGE; s!; des.
+    + pose proof (CHAR1 _ IN_EDGE) as [[SRC_LO SRC_HI] _]. simpl in SRC. lia.
+    + pose proof (CHAR2 _ IN_EDGE) as [[SRC_LO SRC_HI] [DST_LO DST_HI]].
+      assert (RANGE_STEP : qf1 + 1 <= q1 <= qf2) by lia.
+      pose proof (IHDELTA RANGE_STEP ACCEPT) as (s1 & s2 & EQ & DELTA1 & DELTA2).
+      exists (edge.(char_edge_label) :: s1), s2. splits; auto.
+      * rewrite EQ. simpl. now rewrite LABEL.
+      * eapply delta_star_char with (q1 := q1); auto.
+        rewrite <- DST. rewrite <- SRC. eapply char_step_from_edges_complete. exact IN_EDGE.
+Qed.
+
+Lemma regex2fragment_Append_delta_star_start qi qf frag e1 e2 s
+  (REGEX : regex2fragment (Re.Append e1 e2) qi = (qf, frag))
+  (DELTA : frag.(frag_accept) \in fragment_delta_star frag frag.(frag_start) s)
+  : exists qf1, exists frag1, exists qf2, exists frag2, regex2fragment e1 (qi + 1) = (qf1, frag1) /\ regex2fragment e2 (qf1 + 1) = (qf2, frag2) /\ frag.(frag_accept) \in fragment_delta_star frag (qi + 1) s.
+Proof.
+  simpl in REGEX. destruct (regex2fragment e1 (qi + 1)) as [qf1 frag1] eqn: REGEX1. destruct (regex2fragment e2 (qf1 + 1)) as [qf2 frag2] eqn: REGEX2. inv REGEX.
+  exists qf1, frag1, qf2, frag2. splits; eauto.
+  pose proof (regex2fragment_bounds _ _ _ _ REGEX1) as [_ _ LT1 EPS1 CHAR1].
+  pose proof (regex2fragment_bounds _ _ _ _ REGEX2) as [_ _ LT2 EPS2 CHAR2].
+  pose proof (fragment_delta_star_elim_with_src _ _ _ _ DELTA) as [NIL | [EPS | CHAR]].
+  - des; simpl in *; exfalso; lia.
+  - destruct EPS as (q1 & IN_EDGE & REST). simpl in IN_EDGE; s!; des; subst.
+    + exact REST.
+    + exfalso; lia.
+    + exfalso; lia.
+    + pose proof (EPS1 _ IN_EDGE). unfold eps_edge_in_range in *. simpl in *. exfalso; lia.
+    + pose proof (EPS2 _ IN_EDGE). unfold eps_edge_in_range in *. simpl in *. exfalso; lia.
+  - destruct CHAR as (edge & s' & EQ & SRC & IN_EDGE & REST). simpl in IN_EDGE; s!; des.
+    + pose proof (CHAR1 _ IN_EDGE) as [[SRC_LO SRC_HI] _]. simpl in SRC. exfalso; lia.
+    + pose proof (CHAR2 _ IN_EDGE) as [[SRC_LO SRC_HI] _]. simpl in SRC. exfalso; lia.
+Qed.
+
+Lemma regex2fragment_Append_left_delta_star_split qi qf frag e1 e2 qf1 frag1 qf2 frag2 q q' s
+  (REGEX : regex2fragment (Re.Append e1 e2) qi = (qf, frag))
+  (REGEX1 : regex2fragment e1 (qi + 1) = (qf1, frag1))
+  (REGEX2 : regex2fragment e2 (qf1 + 1) = (qf2, frag2))
+  (RANGE : qi + 1 <= q <= qf1)
+  (DELTA : q' \in fragment_delta_star frag q s)
+  (ACCEPT : q' = frag.(frag_accept))
+  : exists s1, exists s2, s = s1 ++ s2 /\ qf1 \in fragment_delta_star frag1 q s1 /\ frag.(frag_accept) \in fragment_delta_star frag (qf1 + 1) s2.
+Proof.
+  revert q q' s RANGE DELTA ACCEPT. simpl in REGEX. rewrite REGEX1 in REGEX. rewrite REGEX2 in REGEX. inv REGEX. intros q q' s RANGE DELTA ACCEPT.
+  pose proof (regex2fragment_bounds _ _ _ _ REGEX1) as [_ _ LT1 EPS1 CHAR1].
+  pose proof (regex2fragment_bounds _ _ _ _ REGEX2) as [_ _ LT2 EPS2 CHAR2].
+  induction DELTA.
+  - simpl in *. exfalso; lia.
+  - pose proof (eps_step_from_edges_sound _ _ _ STEP) as IN_EDGE. s!; des; subst; try now exfalso; lia.
+    + exists [], s. ss!.
+    + pose proof (EPS1 _ IN_EDGE) as [[SRC_LO SRC_HI] [DST_LO DST_HI]]; simpl in SRC_LO, SRC_HI, DST_LO, DST_HI.
+      assert (RANGE_STEP : qi + 1 <= q1 <= qf1) by lia.
+      pose proof (IHDELTA RANGE_STEP eq_refl) as (s1 & s2 & EQ & DELTA1 & DELTA2).
+      exists s1, s2. splits; eauto. eapply delta_star_eps; eauto. eapply eps_step_from_edges_complete; eauto.
+    + pose proof (EPS2 _ IN_EDGE) as [[SRC_LO SRC_HI] _]. simpl in *. exfalso; lia.
+  - pose proof (char_step_from_edges_sound _ _ _ _ STEP) as (edge & IN_EDGE & SRC & LABEL & DST); simpl in IN_EDGE; s!; des.
+    + pose proof (CHAR1 _ IN_EDGE) as [[SRC_LO SRC_HI] [DST_LO DST_HI]].
+      assert (RANGE_STEP : qi + 1 <= q1 <= qf1) by lia.
+      pose proof (IHDELTA RANGE_STEP ACCEPT) as (s1 & s2 & EQ & DELTA1 & DELTA2).
+      exists (edge.(char_edge_label) :: s1), s2. splits; eauto.
+      * rewrite EQ. simpl. now rewrite LABEL.
+      * eapply delta_star_char with (q1 := q1); eauto.
+        rewrite <- DST. rewrite <- SRC. eapply char_step_from_edges_complete; eauto.
+    + pose proof (CHAR2 _ IN_EDGE) as [[SRC_LO SRC_HI] _]. simpl in SRC. exfalso; lia.
+Qed.
+
+Lemma regex2fragment_Append_right_delta_star_split qi qf frag e1 e2 qf1 frag1 qf2 frag2 q q' s
+  (REGEX : regex2fragment (Re.Append e1 e2) qi = (qf, frag))
+  (REGEX1 : regex2fragment e1 (qi + 1) = (qf1, frag1))
+  (REGEX2 : regex2fragment e2 (qf1 + 1) = (qf2, frag2))
+  (RANGE : qf1 + 1 <= q <= qf2)
+  (DELTA : q' \in fragment_delta_star frag q s)
+  (ACCEPT : q' = frag.(frag_accept))
+  : exists s1, exists s2, s = s1 ++ s2 /\ qf2 \in fragment_delta_star frag2 q s1 /\ frag.(frag_accept) \in fragment_delta_star frag frag.(frag_accept) s2.
+Proof.
+  revert q q' s RANGE DELTA ACCEPT; simpl in REGEX. rewrite -> REGEX1, -> REGEX2 in REGEX. inv REGEX; ii.
+  pose proof (regex2fragment_bounds _ _ _ _ REGEX1) as [_ _ LT1 EPS1 CHAR1].
+  pose proof (regex2fragment_bounds _ _ _ _ REGEX2) as [_ _ LT2 EPS2 CHAR2].
+  induction DELTA.
+  - simpl in *. exfalso; lia.
+  - pose proof (eps_step_from_edges_sound _ _ _ STEP) as IN_EDGE. simpl in IN_EDGE. s!; des; subst.
+    + exfalso; lia.
+    + exfalso; lia.
+    + exists [], s. ss!.
+    + pose proof (EPS1 _ IN_EDGE) as [[SRC_LO SRC_HI] _]. simpl in *. exfalso; lia.
+    + pose proof (EPS2 _ IN_EDGE) as [[SRC_LO SRC_HI] [DST_LO DST_HI]].
+      simpl in SRC_LO, SRC_HI, DST_LO, DST_HI.
+      assert (RANGE_STEP : qf1 + 1 <= q1 <= qf2) by lia.
+      pose proof (IHDELTA RANGE_STEP eq_refl) as (s1 & s2 & EQ & DELTA1 & DELTA2).
+      exists s1, s2. splits; eauto. eapply delta_star_eps; eauto. eapply eps_step_from_edges_complete; eauto.
+  - pose proof (char_step_from_edges_sound _ _ _ _ STEP) as (edge & IN_EDGE & SRC & LABEL & DST).
+    simpl in IN_EDGE. rewrite in_app_iff in IN_EDGE. destruct IN_EDGE as [IN_EDGE | IN_EDGE].
+    + pose proof (CHAR1 _ IN_EDGE) as [[SRC_LO SRC_HI] _]. simpl in SRC. lia.
+    + pose proof (CHAR2 _ IN_EDGE) as [[SRC_LO SRC_HI] [DST_LO DST_HI]].
+      assert (RANGE_STEP : qf1 + 1 <= q1 <= qf2) by lia.
+      pose proof (IHDELTA RANGE_STEP ACCEPT) as (s1 & s2 & EQ & DELTA1 & DELTA2).
+      exists (edge.(char_edge_label) :: s1), s2. splits; eauto.
+      * rewrite EQ. simpl. now rewrite LABEL.
+      * eapply delta_star_char with (q1 := q1); eauto.
+        rewrite <- DST. rewrite <- SRC. eapply char_step_from_edges_complete; eauto.
+Qed.
+
+Lemma regex2fragment_Star_delta_star_start qi qf frag e s
+  (REGEX : regex2fragment (Re.Star e) qi = (qf, frag))
+  (DELTA : frag.(frag_accept) \in fragment_delta_star frag frag.(frag_start) s)
+  : exists qf1, exists frag1, regex2fragment e (qi + 1) = (qf1, frag1) /\ frag.(frag_accept) \in fragment_delta_star frag (qi + 1) s.
+Proof.
+  simpl in REGEX. destruct (regex2fragment e (qi + 1)) as [qf1 frag1] eqn: REGEX1.
+  inv REGEX. exists qf1, frag1. split; eauto.
+  pose proof (regex2fragment_bounds _ _ _ _ REGEX1) as [_ _ LT1 EPS1 CHAR1].
+  pose proof (fragment_delta_star_elim_with_src _ _ _ _ DELTA) as [NIL | [EPS | CHAR]].
+  - des; simpl in *; exfalso; lia.
+  - destruct EPS as (q1 & IN_EDGE & REST). simpl in IN_EDGE; s!; des; subst.
+    + exact REST.
+    + exfalso; lia.
+    + exfalso; lia.
+    + pose proof (EPS1 _ IN_EDGE). unfold eps_edge_in_range in *. simpl in *. exfalso; lia.
+  - destruct CHAR as (edge & s' & EQ & SRC & IN_EDGE & REST).
+    pose proof (CHAR1 _ IN_EDGE) as [[SRC_LO SRC_HI] _]. simpl in SRC. exfalso; lia.
+Qed.
+
+Lemma regex2fragment_accept_delta_star_stuck e qi qf frag q' s
+  (REGEX : regex2fragment e qi = (qf, frag))
+  (DELTA : q' \in fragment_delta_star frag qf s)
+  : s = [] /\ q' = qf.
+Proof.
+  eapply delta_star_stuck; eauto.
+  - intros q IN. pose proof (eps_step_from_edges_sound _ _ _ IN) as IN_EDGE.
+    pose proof (regex2fragment_edge_src_lt _ _ _ _ REGEX) as [EPS _]. done!.
+  - intros c q IN. pose proof (char_step_from_edges_sound _ _ _ _ IN) as (edge & IN_EDGE & SRC & LABEL & DST).
+    pose proof (regex2fragment_edge_src_lt _ _ _ _ REGEX) as [_ CHAR]. done!.
+Qed.
+
+Lemma regex2fragment_Star_delta_star_sound_aux e
+  (SOUND : forall qi, forall qf, forall frag, forall s, regex2fragment e qi = (qf, frag) -> frag.(frag_accept) \in fragment_delta_star frag frag.(frag_start) s -> s \in eval_regex e)
+  : forall qi, forall qf, forall frag, forall qf1, forall frag1, forall q, forall q', forall s, regex2fragment (Re.Star e) qi = (qf, frag) -> regex2fragment e (qi + 1) = (qf1, frag1) -> qi + 1 <= q <= qf1 -> q' \in fragment_delta_star frag q s -> q' = frag.(frag_accept) ->  ((s = [] /\ q = qi + 1) \/ (exists s1, exists s2, s = s1 ++ s2 /\ qf1 \in fragment_delta_star frag1 q s1 /\ s2 \in eval_regex (Re.Star e))).
+Proof.
+  ii. revert q q' s H1 H2 H3. simpl in H. rewrite H0 in H. inv H. intros q q' s RANGE DELTA ACCEPT.
+  pose proof (regex2fragment_bounds _ _ _ _ H0) as [START1 ACCEPT1 LT1 EPS1 CHAR1].
+  pose proof (regex2fragment_edge_dst_gt_start _ _ _ _ H0) as [EPS_DST CHAR_DST].
+  induction DELTA.
+  - simpl in *; exfalso; lia.
+  - pose proof (eps_step_from_edges_sound _ _ _ STEP) as IN_EDGE. simpl in IN_EDGE; s!; des; subst.
+    + exfalso; lia.
+    + set (qf1 := frag_accept frag1).
+      enough (STAR_IN : s \in eval_regex (Re.Star e)).
+      { right. exists [], s. ss!. }
+      assert (RANGE_STEP : qi + 1 <= qi + 1 <= qf1) by lia.
+      pose proof (IHDELTA RANGE_STEP eq_refl) as [[EQ _] | (s1 & s2 & EQ & DELTA1 & STAR)]; subst; simpl; [econs 1 | econs 2]; eauto.
+      eapply SOUND; eauto. rewrite START1; eauto.
+    + set (qf1 := frag_accept frag1).
+      assert (REGEX_STAR : regex2fragment (Re.Star e) qi = (frag_accept frag1 + 1, mkFragment qi (qf1 + 1) ((qi, qi + 1) :: (qf1, qi + 1) :: (qi + 1, qf1 + 1) :: frag1.(frag_eps_edges)) frag1.(frag_char_edges))) by now simpl; rewrite H0.
+      pose proof (regex2fragment_accept_delta_star_stuck (Re.Star e) qi (qf1 + 1) (mkFragment qi (qf1 + 1) ((qi, qi + 1) :: (qf1, qi + 1) :: (qi + 1, qf1 + 1) :: frag1.(frag_eps_edges)) frag1.(frag_char_edges)) _ s REGEX_STAR REST) as [EQ _]; subst s.
+      left; ss!.
+    + set (qf1 := frag_accept frag1).
+      pose proof (EPS1 _ IN_EDGE) as [[SRC_LO SRC_HI] [DST_LO DST_HI]]; simpl in SRC_LO, SRC_HI, DST_LO, DST_HI.
+      assert (RANGE_STEP : qi + 1 <= q1 <= qf1) by lia.
+      pose proof (IHDELTA RANGE_STEP eq_refl) as [[EQ EQ'] | (s1 & s2 & EQ & DELTA1 & STAR)]; subst.
+      * pose proof (EPS_DST _ _ IN_EDGE); done!.
+      * right. exists s1, s2. splits; eauto.
+        eapply delta_star_eps; eauto. eapply eps_step_from_edges_complete; eauto.
+  - pose proof (char_step_from_edges_sound _ _ _ _ STEP) as (edge & IN_EDGE & SRC & LABEL & DST).
+    pose proof (CHAR1 _ IN_EDGE) as [[SRC_LO SRC_HI] [DST_LO DST_HI]].
+    assert (RANGE_STEP : qi + 1 <= q1 <= qf1) by lia.
+    pose proof (IHDELTA RANGE_STEP ACCEPT) as [[EQ EQ'] | (s1 & s2 & EQ & DELTA1 & STAR)]; subst.
+    + pose proof (CHAR_DST _ IN_EDGE); done!.
+    + right. exists (edge.(char_edge_label) :: s1), s2. splits; eauto. econs 3; eauto.
+Qed.
+
+Theorem regex2fragment_sound_Null qi qf frag s
+  (REGEX : regex2fragment Re.Null qi = (qf, frag))
+  (DELTA : frag.(frag_accept) \in fragment_delta_star frag frag.(frag_start) s)
+  : s \in eval_regex Re.Null.
+Proof.
+  simpl in REGEX. inv REGEX. pose proof (fragment_delta_star_elim _ _ _ _ DELTA) as [NIL | [EPS | CHAR]].
+  - des; simpl in *; exfalso; lia.
+  - des; contradiction.
+  - des; contradiction.
+Qed.
+
+Theorem regex2fragment_sound_Empty qi qf frag s
+  (REGEX : regex2fragment Re.Empty qi = (qf, frag))
+  (DELTA : frag.(frag_accept) \in fragment_delta_star frag frag.(frag_start) s)
+  : s \in eval_regex Re.Empty.
+Proof.
+  simpl in REGEX. inv REGEX. pose proof (fragment_delta_star_elim _ _ _ _ DELTA) as [NIL | [EPS | CHAR]].
+  - des; simpl in *; exfalso; lia.
+  - destruct EPS as (q1 & IN_EDGE & REST). simpl in IN_EDGE.
+    destruct IN_EDGE as [EQ | []]. inv EQ.
+    pose proof (regex2fragment_accept_delta_star_stuck Re.Empty qi (qi + 1) (mkFragment qi (qi + 1) [(qi, qi + 1)] []) (qi + 1) s eq_refl REST) as [EQ ?]; subst s.
+    ss!.
+  - des; contradiction.
+Qed.
+
+Theorem regex2fragment_sound_Char c qi qf frag s
+  (REGEX : regex2fragment (Re.Char c) qi = (qf, frag))
+  (DELTA : frag.(frag_accept) \in fragment_delta_star frag frag.(frag_start) s)
+  : s \in eval_regex (Re.Char c).
+Proof.
+  simpl in REGEX. inv REGEX. pose proof (fragment_delta_star_elim _ _ _ _ DELTA) as [NIL | [EPS | CHAR]].
+  - des; simpl in *; exfalso; lia.
+  - des; contradiction.
+  - destruct CHAR as (edge & s' & EQ & IN_EDGE & REST). simpl in IN_EDGE.
+    destruct IN_EDGE as [EDGE_EQ | []]. subst edge. simpl in EQ. subst s.
+    pose proof (regex2fragment_accept_delta_star_stuck (Re.Char c) qi (qi + 1) (mkFragment qi (qi + 1) [] [mkCharEdge qi c (qi + 1)]) (qi + 1) s' eq_refl REST) as [EQ ?]; subst s'.
+    ss!.
+Qed.
+
+Theorem regex2fragment_sound_Union e1 e2
+  (SOUND1 : forall qi, forall qf, forall frag, forall s, regex2fragment e1 qi = (qf, frag) -> frag.(frag_accept) \in fragment_delta_star frag frag.(frag_start) s -> s \in eval_regex e1)
+  (SOUND2 : forall qi, forall qf, forall frag, forall s, regex2fragment e2 qi = (qf, frag) -> frag.(frag_accept) \in fragment_delta_star frag frag.(frag_start) s -> s \in eval_regex e2)
+  : forall qi, forall qf, forall frag, forall s, regex2fragment (Re.Union e1 e2) qi = (qf, frag) -> frag.(frag_accept) \in fragment_delta_star frag frag.(frag_start) s -> s \in eval_regex (Re.Union e1 e2).
+Proof.
+  ii. pose proof (regex2fragment_start_accept _ _ _ _ H) as [_ ACCEPT]. pose proof (regex2fragment_Union_delta_star_start qi qf frag e1 e2 s H H0) as (qf1 & frag1 & qf2 & frag2 & REGEX1 & REGEX2 & [DELTA1 | DELTA2]).
+  - pose proof (regex2fragment_bounds _ _ _ _ REGEX1) as [START1 ACCEPT1 LT1 _ _].
+    assert (RANGE1 : qi + 1 <= qi + 1 <= qf1) by lia.
+    pose proof (regex2fragment_Union_left_delta_star_split qi qf frag e1 e2 qf1 frag1 qf2 frag2 (qi + 1) frag.(frag_accept) s H REGEX1 REGEX2 RANGE1 DELTA1 eq_refl) as (s1 & s2 & EQ & DELTA1' & DELTA2').
+    rewrite ACCEPT in DELTA2'.
+    pose proof (regex2fragment_accept_delta_star_stuck (Re.Union e1 e2) qi qf frag qf s2 H DELTA2') as [EQ2 _]; subst s2.
+    rewrite app_nil_r in EQ; subst s. s!. left. eapply SOUND1; done!.
+  - pose proof (regex2fragment_bounds _ _ _ _ REGEX2) as [START2 ACCEPT2 LT2 _ _].
+    assert (RANGE2 : qf1 + 1 <= qf1 + 1 <= qf2) by lia.
+    pose proof (regex2fragment_Union_right_delta_star_split qi qf frag e1 e2 qf1 frag1 qf2 frag2 (qf1 + 1) frag.(frag_accept) s H REGEX1 REGEX2 RANGE2 DELTA2 eq_refl) as (s1 & s2 & EQ & DELTA1' & DELTA2').
+    rewrite ACCEPT in DELTA2'.
+    pose proof (regex2fragment_accept_delta_star_stuck (Re.Union e1 e2) qi qf frag qf s2 H DELTA2') as [EQ2 _]; subst s2.
+    rewrite app_nil_r in EQ; subst s. s!. right. eapply SOUND2; done!.
+Qed.
+
+Theorem regex2fragment_sound_Append e1 e2
+  (SOUND1 : forall qi, forall qf, forall frag, forall s, regex2fragment e1 qi = (qf, frag) -> frag.(frag_accept) \in fragment_delta_star frag frag.(frag_start) s -> s \in eval_regex e1)
+  (SOUND2 : forall qi, forall qf, forall frag, forall s, regex2fragment e2 qi = (qf, frag) -> frag.(frag_accept) \in fragment_delta_star frag frag.(frag_start) s -> s \in eval_regex e2)
+  : forall qi, forall qf, forall frag, forall s, regex2fragment (Re.Append e1 e2) qi = (qf, frag) -> frag.(frag_accept) \in fragment_delta_star frag frag.(frag_start) s -> s \in eval_regex (Re.Append e1 e2).
+Proof.
+  ii. pose proof (regex2fragment_start_accept _ _ _ _ H) as [_ ACCEPT].
+  pose proof (regex2fragment_Append_delta_star_start qi qf frag e1 e2 s H H0) as (qf1 & frag1 & qf2 & frag2 & REGEX1 & REGEX2 & DELTA).
+  pose proof (regex2fragment_bounds _ _ _ _ REGEX1) as [START1 ACCEPT1 LT1 _ _].
+  pose proof (regex2fragment_bounds _ _ _ _ REGEX2) as [START2 ACCEPT2 LT2 _ _].
+  assert (RANGE1 : qi + 1 <= qi + 1 <= qf1) by lia.
+  assert (RANGE2 : qf1 + 1 <= qf1 + 1 <= qf2) by lia.
+  pose proof (regex2fragment_Append_left_delta_star_split qi qf frag e1 e2 qf1 frag1 qf2 frag2 (qi + 1) frag.(frag_accept) s H REGEX1 REGEX2 RANGE1 DELTA eq_refl) as (s1 & s2 & EQ & DELTA1 & DELTA2).
+  pose proof (regex2fragment_Append_right_delta_star_split qi qf frag e1 e2 qf1 frag1 qf2 frag2 (qf1 + 1) frag.(frag_accept) s2 H REGEX1 REGEX2 RANGE2 DELTA2 eq_refl) as (s2' & s3 & EQ' & DELTA2' & DELTA3).
+  rewrite ACCEPT in DELTA3.
+  pose proof (regex2fragment_accept_delta_star_stuck (Re.Append e1 e2) qi qf frag qf s3 H DELTA3) as [EQ3 _]; subst s3.
+  rewrite app_nil_r in EQ'; subst s2 s; simpl.
+  exists s1; split.
+  { eapply SOUND1; done!. }
+  exists s2'. split.
+  { eapply SOUND2; done!. }
+  red; reflexivity.
+Qed.
+
+Theorem regex2fragment_sound_Star e1
+  (SOUND : forall qi, forall qf, forall frag, forall s, regex2fragment e1 qi = (qf, frag) -> frag.(frag_accept) \in fragment_delta_star frag frag.(frag_start) s -> s \in eval_regex e1)
+  : forall qi, forall qf, forall frag, forall s, regex2fragment (Re.Star e1) qi = (qf, frag) -> frag.(frag_accept) \in fragment_delta_star frag frag.(frag_start) s -> s \in eval_regex (Re.Star e1).
+Proof.
+  ii. pose proof (regex2fragment_Star_delta_star_start qi qf frag e1 s H H0) as (qf1 & frag1 & REGEX & DELTA).
+  pose proof (regex2fragment_bounds _ _ _ _ REGEX) as [START ACCEPT LT _ _].
+  assert (RANGE : qi + 1 <= qi + 1 <= qf1) by lia.
+  pose proof (regex2fragment_Star_delta_star_sound_aux e1 SOUND qi qf frag qf1 frag1 (qi + 1) frag.(frag_accept) s H REGEX RANGE DELTA eq_refl) as [[EQ _] | (s1 & s2 & EQ & DELTA1 & STAR)]; subst s; simpl; [econs 1 | econs 2].
+  - eapply SOUND; done!.
+  - exact STAR.
+Qed.
+
+Corollary regex2fragment_sound (e : regex ascii)
+  : forall qi, forall qf, forall frag, forall s, regex2fragment e qi = (qf, frag) -> frag.(frag_accept) \in fragment_delta_star frag frag.(frag_start) s -> s \in eval_regex e.
+Proof.
+  induction e.
+  - now eapply regex2fragment_sound_Null.
+  - now eapply regex2fragment_sound_Empty.
+  - now eapply regex2fragment_sound_Char.
+  - now eapply regex2fragment_sound_Union.
+  - now eapply regex2fragment_sound_Append.
+  - now eapply regex2fragment_sound_Star.
+Qed.
+
+Lemma fragments_delta_star_start_to_fragment qi rules qmax frags rule frag qi_rule qf s
+  (FRAGS : rules2fragments qi rules = (qmax, frags))
+  (IN_FRAG : (rule, frag) ∈ frags)
+  (REGEX : regex2fragment rule.(Rule.regex) qi_rule = (qf, frag))
+  (qi_POS : 0 < qi)
+  (DELTA : frag.(frag_accept) \in fragments_delta_star frags 0 s)
+  : frag.(frag_accept) \in fragment_delta_star frag frag.(frag_start) s.
+Proof.
+  pose proof (regex2fragment_bounds _ _ _ _ REGEX) as [START ACCEPT LT _ _].
+  pose proof (delta_star_elim _ _ 0 frag.(frag_accept) s DELTA) as [NIL | [EPS | CHAR]].
+  - des; subst.
+    pose proof (rules2fragments_start_ge _ _ _ _ _ _ _ _ FRAGS IN_FRAG REGEX); done!.
+  - destruct EPS as (q1 & STEP & REST).
+    pose proof (eps_step_from_edges_sound _ _ _ STEP) as IN_EDGE.
+    pose proof (fragment_eps_edges_start_sound _ _ _ _ _ FRAGS qi_POS IN_EDGE) as (rule' & frag' & qi_rule' & qf' & IN_FRAG' & REGEX' & START_EDGE); subst q1.
+    pose proof (regex2fragment_bounds _ _ _ _ REGEX') as [START' ACCEPT' LT' _ _].
+    assert (RANGE : qi_rule <= frag.(frag_accept) <= qf) by lia.
+    assert (RANGE' : qi_rule' <= frag.(frag_accept) <= qf').
+    { eapply delta_star_fragment_range with (qi := qi) (rules := rules) (qmax := qmax) (frags := frags) (rule := rule') (frag := frag') (q := frag'.(frag_start)) (s := s); done!. }
+    pose proof (rules2fragments_ranges_disjoint _ _ _ _ _ _ _ _ _ _ _ _ _ FRAGS IN_FRAG IN_FRAG' REGEX REGEX' RANGE RANGE') as EQ.
+    eapply delta_star_global_to_fragment; done!.
+  - destruct CHAR as (c & s' & q1 & EQ & STEP & REST).
+    pose proof (char_step_from_edges_sound _ _ _ _ STEP) as (edge & IN_EDGE & SRC & LABEL & DST).
+    pose proof (fragment_char_edges_owner _ _ _ _ _ FRAGS IN_EDGE) as (rule' & frag' & qi_rule' & qf' & IN_FRAG' & REGEX' & BOUNDS' & LE_START & LT_END & RANGE' & IN_EDGE').
+    done!.
+Qed.
+
+Lemma TaggedENFA_FRAGMENTS_sound qi rules qmax frags s tag
+  (FRAGS : rules2fragments qi rules = (qmax, frags))
+  (qi_POS : 0 < qi)
+  (ACCEPTS : accepts (fragments2TaggedENFA qmax frags) s tag)
+  : exists rule, rule ∈ rules /\ rule.(Rule.token) = tag /\ s \in eval_regex rule.(Rule.regex).
+Proof.
+  destruct ACCEPTS as (q & DELTA & ACCEPT). simpl in DELTA, ACCEPT.
+  pose proof (fragment_accept_states_sound _ _ _ ACCEPT) as (rule & frag & IN_FRAG & ACCEPT_EQ & TOKEN_EQ); subst q tag.
+  pose proof (rules2fragments_bounds _ _ _ _ FRAGS) as [_ BOUND].
+  pose proof (BOUND _ _ IN_FRAG) as (qi_rule & qf & REGEX & _ & _ & _).
+  exists rule. split.
+  - eapply rules2fragments_sound; eauto.
+  - split; eauto. eapply regex2fragment_sound; eauto. eapply fragments_delta_star_start_to_fragment; eauto.
+Qed.
+
+Theorem mkUnitedTaggedENFA_sound (M : TaggedENFA.t)
+  (COMPILE : fmap mkUnitedTaggedENFA Rule.compileds = inr M)
+  : exists rules, Rule.compileds = inr rules /\ ⟪ ACCEPT : forall s, forall tag, accepts M s tag -> (exists rule, rule ∈ rules /\ rule.(Rule.token) = tag /\ s \in eval_regex rule.(Rule.regex)) ⟫.
+Proof.
+  pose proof (mkUnitedTaggedENFA_spec M COMPILE) as (rules & qmax & frags & COMPILED & FRAGMENTS_OF).
+  destruct COMPILED as [COMPILED_RULES COMPILED_ENFA COMPILED_FRAGS].
+  exists rules. split; [exact COMPILED_RULES | unnw]. intros s tag ACCEPTS.
+  assert (ENFA_EQ : M = fragments2TaggedENFA qmax frags).
+  { eapply TaggedENFA_COMPILED_as_fragments. econs; eauto. }
+  rewrite ENFA_EQ in ACCEPTS. eapply TaggedENFA_FRAGMENTS_sound; eauto.
+Qed.
+
+Theorem mkUnitedTaggedENFA_complete (M : TaggedENFA.t)
+  (COMPILE : fmap mkUnitedTaggedENFA Rule.compileds = inr M)
+  : exists rules, Rule.compileds = inr rules /\ ⟪ ACCEPT : forall s, forall tag, (exists rule, rule ∈ rules /\ rule.(Rule.token) = tag /\ s \in eval_regex rule.(Rule.regex)) -> accepts M s tag ⟫.
+Proof.
+  pose proof (mkUnitedTaggedENFA_spec M COMPILE) as (rules & qmax & frags & COMPILED & FRAGMENTS_OF).
+  destruct COMPILED as [COMPILED_RULES COMPILED_ENFA COMPILED_FRAGS].
+  exists rules. split; [exact COMPILED_RULES | unnw]. intros s tag (rule & IN_RULE & TOKEN & IN_REGEX); subst tag.
+  pose proof (rules2fragments_complete 1 rules qmax frags rule COMPILED_FRAGS IN_RULE) as (qi & qf & frag & REGEX2FRAGMENT & IN_FRAGS).
+  pose proof (FRAGMENTS_OF rule frag IN_FRAGS) as FRAGMENTS.
+  pose proof (TaggedENFA_FRAGMENTS_complete qmax frags rule qi qf frag s REGEX2FRAGMENT FRAGMENTS IN_REGEX) as ACCEPTS.
+  rewrite TaggedENFA_COMPILED_as_fragments with (M := M) (rules := rules) (qmax := qmax) (frags := frags); eauto.
+  exact (TaggedENFA_COMPILED_intro M rules qmax frags COMPILED_RULES COMPILED_ENFA COMPILED_FRAGS).
+Qed.
+
+End Thompson's_construction.
+
+Module Thompson.
+
+Definition accepts_global (frags : list (Rule.t * fragment)) (frag : fragment) (s : Input.t) : Prop :=
+  frag.(frag_accept) \in fragments_delta_star frags frag.(frag_start) s.
+
+Definition accepts_local (frag : fragment) (s : Input.t) : Prop :=
+  frag.(frag_accept) \in fragment_delta_star frag frag.(frag_start) s.
+
+Theorem regex2fragment_invariant (e : regex ascii) (qi : nat) (qf : nat) (frag : fragment)
+  (REGEX : regex2fragment e qi = (qf, frag))
+  : FRAGMENT_BOUNDS qi qf frag.
+Proof.
+  now eapply regex2fragment_bounds with (e := e).
+Qed.
+
+Theorem regex2fragment_start_accept (e : regex ascii) (qi : nat) (qf : nat) (frag : fragment)
+  (REGEX : regex2fragment e qi = (qf, frag))
+  : frag.(frag_start) = qi /\ frag.(frag_accept) = qf.
+Proof.
+  now eapply TaggedENFA.regex2fragment_start_accept with (e := e).
+Qed.
+
+Variant REGEX2FRAGMENT_CORRECT (frags : list (Rule.t * fragment)) (rule : Rule.t) (qi : nat) (qf : nat) (frag : fragment) : Prop :=
+  | regex2fragment_correct_intro
+    (regex2fragment_local_sound : forall s : Input.t, frag.(frag_accept) \in fragment_delta_star frag frag.(frag_start) s -> s \in eval_regex rule.(Rule.regex))
+    (regex2fragment_global_complete : forall s : Input.t, s \in eval_regex rule.(Rule.regex) -> frag.(frag_accept) \in fragments_delta_star frags frag.(frag_start) s).
+
+Theorem regex2fragment_correct frags rule qi qf frag
+  (REGEX : regex2fragment rule.(Rule.regex) qi = (qf, frag))
+  (FRAGMENTS : TaggedENFA_FRAGMENTS frags rule frag)
+  : REGEX2FRAGMENT_CORRECT frags rule qi qf frag.
+Proof.
+  constructor.
+  - intros s ACCEPT. eapply regex2fragment_sound; eauto.
+  - intros s ACCEPT. eapply regex2fragment_complete; eauto.
+Qed.
+
+Theorem mkUnitedTaggedENFA_correct (M : TaggedENFA.t)
+  (COMPILE : fmap mkUnitedTaggedENFA Rule.compileds = inr M)
+  : exists rules, Rule.compileds = inr rules /\ ⟪ CORRECT : forall s, forall tag, accepts M s tag <-> exists rule, rule ∈ rules /\ rule.(Rule.token) = tag /\ s \in eval_regex rule.(Rule.regex) ⟫.
+Proof.
+  pose proof (TaggedENFA.mkUnitedTaggedENFA_sound M COMPILE) as (rules & COMPILED & SOUND); unnw.
+  pose proof (TaggedENFA.mkUnitedTaggedENFA_complete M COMPILE) as (rules' & COMPILED' & COMPLETE); unnw.
+  rewrite COMPILED in COMPILED'. inv COMPILED'. exists rules'; ss!.
+Qed.
+
+End Thompson.
+
+End TaggedENFA.
 
 End MkLGS.
